Soundness proof for locals

ch2o_compcertc_lp64.v
@@ -1,5 +1,5 @@
 From ch2o_compcert Require Export ch2o_safety compcertc_safety.
-From ch2o Require Export stringmap types expressions statements architectures state.
+From ch2o Require Export stringmap types expressions statements architectures architecture_spec state.
 (* We prove soundness for LP64 architectures. *)
 From ch2o_compcert Require Export ch2o_lp64.
 From compcert Require Export Cop Csyntax Ctypes Globalenvs.
@@ -10,94 +10,59 @@ Section Program.
 
 Local Open Scope string_scope.
 
-Context (Γ: types.env K) (δ: funenv K) (p: Csyntax.program).
+Context (Γ: types.env K) (δ: funenv K) (p: Csyntax.program) (valid_Γ: ✓ Γ).
 
-Inductive expr_equiv: expressions.expr K → Csyntax.expr → Prop :=
-| expr_equiv_val_int z:
+Notation tint := (Tint I32 Signed noattr).
+
+Inductive type_ := Int | Loc.
+
+Section Locals.
+
+Context (ê: list AST.ident).
+
+Inductive expr_equiv: expressions.expr K → Csyntax.expr → type_ → Prop :=
+| expr_equiv_val_int Ω z:
   int_typed z (sintT: int_type K) → (* TODO: Require the CH2O program to be well-typed instead? *)
-  expr_equiv (EVal ∅ (inr (intV{sintT} z))) (Eval (Vint (Int.repr z)) (Tint I32 Signed noattr))
+  expr_equiv (#{Ω} intV{sintT} z) (Eval (Vint (Int.repr z)) tint) Int
 | expr_equiv_div e1 ė1 e2 ė2:
-  expr_equiv e1 ė1 →
-  expr_equiv e2 ė2 →
-  expr_equiv (e1 / e2) (Ebinop Odiv ė1 ė2 (Tint I32 Signed noattr))
+  expr_equiv e1 ė1 Int →
+  expr_equiv e2 ė2 Int →
+  expr_equiv (e1 / e2) (Ebinop Odiv ė1 ė2 tint) Int
+| expr_equiv_var i x:
+  ê !! i = Some x →
+  expr_equiv (var i) (Evar x tint) Loc
+| expr_equiv_loc b:
+  expr_equiv (%(Ptr (addr_top (Npos b) sintT))) (Eloc b Ptrofs.zero tint) Loc
+| expr_equiv_load e ė:
+  expr_equiv e ė Loc →
+  expr_equiv (load e)%E (Evalof ė tint) Int
+| expr_equiv_val_indet:
+  expr_equiv (# indetV sintT) (Eval Vundef tint) Int
+| expr_equiv_assign e1 ė1 e2 ė2:
+  expr_equiv e1 ė1 Loc →
+  expr_equiv e2 ė2 Int →
+  expr_equiv (e1 ::= e2) (Eassign ė1 ė2 tint) Int
 .
 
 Inductive stmt_equiv: stmt K → statement → Prop :=
 | stmt_equiv_return e ė:
-  expr_equiv e ė →
+  expr_equiv e ė Int →
   stmt_equiv (ret (cast{sintT%T} e)) (Sreturn (Some ė))
 | stmt_equiv_skip:
-  stmt_equiv SSkip Sskip
+  stmt_equiv skip Sskip
 | stmt_equiv_sequence s1 ṡ1 s2 ṡ2:
   stmt_equiv s1 ṡ1 →
   stmt_equiv s2 ṡ2 →
-  stmt_equiv (SComp s1 s2) (Ssequence ṡ1 ṡ2)
+  stmt_equiv (s1 ;; s2) (Ssequence ṡ1 ṡ2)
 | stmt_equiv_if e ė s1 ṡ1 s2 ṡ2:
-  expr_equiv e ė →
+  expr_equiv e ė Int →
   stmt_equiv s1 ṡ1 →
   stmt_equiv s2 ṡ2 →
-  stmt_equiv (SIf e s1 s2) (Sifthenelse ė ṡ1 ṡ2)
+  stmt_equiv (if{e} s1 else s2) (Sifthenelse ė ṡ1 ṡ2)
+| stmt_equiv_do e ė:
+  expr_equiv e ė Int →
+  stmt_equiv (! (cast{voidT%T} e)) (Sdo ė)
 .
-
-Inductive program_equiv: Prop :=
-| program_equiv_intro s ṡ b:
-  stringmap_lookup "main" δ = Some s →
-  Genv.init_mem p <> None →
-  let ge := globalenv p in
-  Genv.find_symbol ge p.(prog_main) = Some b →
-  let f := {|
-    fn_return:=type_int32s;
-    fn_callconv:=AST.cc_default;
-    fn_params:=nil;
-    fn_vars:=nil;
-    fn_body:=
-      Ssequence
-        ṡ
-        (Sreturn (Some (Eval (Vint (Int.repr 0)) (Tint I32 Signed noattr))))
-  |} in
-  Genv.find_funct_ptr ge b = Some (Internal f) →
-  stmt_equiv s ṡ →
-  program_equiv.
-
-Fixpoint globdef_is_fun{F V}(g: AST.globdef F V): bool :=
-  match g with
-    AST.Gfun _ => true
-  | AST.Gvar _ => false
-  end.
-
-Lemma init_mem_ok `{prog: Ctypes.program F}:
-  forallb (λ gd, globdef_is_fun (gd.2)) (AST.prog_defs prog) = true →
-  Genv.init_mem prog <> None.
-Proof.
-intros.
-unfold Genv.init_mem.
-assert (∀ gl ge m, (∀ g, In g gl → globdef_is_fun (snd g) = true) → Genv.alloc_globals (F:=Ctypes.fundef F) (V:=type) ge m gl <> None). {
-  induction gl; intros.
-  - simpl. intro; discriminate.
-  - simpl.
-    unfold Genv.alloc_global.
-    destruct a.
-    destruct g.
-    + case_eq (Memory.Mem.alloc m 0 1).
-      intros.
-      destruct (Memory.Mem.range_perm_drop_2 m0 b 0 1 Memtype.Nonempty).
-      * unfold Memory.Mem.range_perm.
-        intros.
-        apply Memory.Mem.perm_alloc_2 with (1:=H1) (2:=H2).
-      * rewrite e.
-        apply IHgl.
-        intros.
-        apply H0.
-        right.
-        assumption.
-    + lapply (H0 (i, AST.Gvar v)).
-      intros; discriminate. left.
-      reflexivity.
-}
-apply H0.
-rewrite -> (List.forallb_forall (A:=AST.ident * AST.globdef (Ctypes.fundef F) type)) in H.
-apply H.
-Qed.
 
 Lemma int_typed_limits z:
   int_typed z (sintT%IT: int_type K) →
@@ -162,6 +127,7 @@ destruct (classic (imm_safe (globalenv p) e RV a m)).
   + eassumption.
 Qed.
 
+(*
 Lemma expr_equiv_no_LV_context e ė:
   expr_equiv e ė →
   ∀ C a,
@@ -177,8 +143,7 @@ induction 1; intros.
   + injection H2; clear H2; intros; subst.
     eelim IHexpr_equiv2 with (1:=H3); reflexivity.
 Qed.
-
-Notation tint := (Tint I32 Signed noattr).
+*)
 
 Lemma sem_cast_int z m:
   sem_cast (Vint (Int.repr z)) tint tint m = Some (Vint (Int.repr z)).
@@ -210,27 +175,692 @@ simpl.
 reflexivity.
 Qed.
 
-Lemma rred_safe e ė:
-  expr_equiv e ė →
-  ∀ C a ẽ ṁ t a' ṁ' ρ m,
-  context RV RV C →
+Definition ch2o_val_of(oz: option Z): val K :=
+  match oz with
+    None => indetV sintT
+  | Some z => intV{sintT} z
+  end.
+
+Definition compcert_val_of(oz: option Z): Values.val :=
+  match oz with
+    None => Vundef
+  | Some z => Vint (Int.repr z)
+  end.
+  
+Lemma mem_lookup_dom m i v:
+  m !!{Γ} addr_top i sintT = Some v → i ∈ dom indexset m.
+Proof.
+  unfold lookupE.
+  unfold mem_lookup.
+  unfold lookupE.
+  unfold cmap_lookup.
+  rewrite option_guard_True. 2:{ constructor. simpl. lia. }
+  unfold lookupE.
+  unfold cmap_lookup_ref.
+  simpl.
+  case_eq (cmap_car m !! i); simpl; intros; try congruence.
+  apply elem_of_dom_2 in H.
+  destruct m.
+  assumption.
+Qed.
+
+Lemma mem_writable_dom i m:
+  mem_writable Γ (addr_top i sintT) m → i ∈ dom indexset m.
+Proof.
+  destruct m as [m].
+  unfold mem_writable.
+  intros.
+  destruct H as [w [? ?]].
+  unfold lookupE in H.
+  unfold cmap_lookup in H.
+  rewrite option_guard_True in H. 2:{ constructor. simpl. lia. }
+  simpl in H.
+  case_eq (m !! i); intros; rewrite H1 in H; try discriminate.
+  apply elem_of_dom_2 in H1.
+  assumption.
+Qed.
+
+Lemma mem_lookup_index_alive m i v:
+  m !!{Γ} addr_top i sintT = Some v → index_alive '{m} i.
+Proof.
+  destruct m as [m]; simpl.
+  unfold mem_lookup; simpl.
+  unfold cmap_lookup.
+  unfold index_alive.
+  rewrite option_guard_True. 2:{ constructor. simpl. lia. }
+  simpl.
+  case_eq (m !! i); simpl; intros; try congruence.
+  destruct c as [|w μ]; simpl in H0; try congruence.
+  exists (type_of w).
+  rewrite lookup_fmap.
+  rewrite H.
+  reflexivity.
+Qed.
+
+Inductive block_equiv(m: memory_map.mem K)(ṁ: Memory.Mem.mem)(b: Values.block): Prop :=
+| block_equiv_not_alloced:
+  (*
+  Memory.Mem.loadv AST.Mint32 ṁ (Vptr b Ptrofs.zero) = None →
+  (∀ v, Memory.Mem.storev AST.Mint32 ṁ (Vptr b Ptrofs.zero) v = None) →
+  Memory.Mem.free ṁ b 0%Z 4%Z = None →
+  m !!{Γ} addr_top (Npos b) sintT = None →
+  ~ mem_writable Γ (addr_top (Npos b) sintT) m →
+  *)
+  ¬ index_alive '{m} (Npos b) →
+  block_equiv m ṁ b
+| block_equiv_alloced oz:
+  Memory.Mem.loadv AST.Mint32 ṁ (Vptr b Ptrofs.zero) = Some (compcert_val_of oz) →
+  Memory.Mem.valid_access ṁ AST.Mint32 b 0 Memtype.Writable →
+  Memory.Mem.range_perm ṁ b 0%Z 4%Z Memtype.Cur Memtype.Freeable →
+  index_alive '{m} (Npos b) →
+  (Γ, '{m}) ⊢ addr_top (N.pos b) sintT : TType sintT%T →
+  m !!{Γ} addr_top (Npos b) sintT = Some (ch2o_val_of oz) →
+  mem_writable Γ (addr_top (Npos b) sintT) m →
+  match oz with None => True | Some z => int_typed z (sintT: int_type K) end →
+  block_equiv m ṁ b
+.
+
+Record mem_equiv(m: memory_map.mem K)(ṁ: Memory.Mem.mem) := {
+  blocks_equiv: ∀ b, block_equiv m ṁ b;
+  domains_equiv: ∀ b, (ṁ.(Memory.Mem.nextblock) ≤ b)%positive → (Npos b : index) ∉ dom indexset m;
+  mem_valid: ✓{Γ} m
+}.
+
+Lemma mem_equiv_insert m ṁ b z ṁ':
+  mem_equiv m ṁ →
+  (Γ, '{m}) ⊢ addr_top (N.pos b) sintT : TType sintT%T →
+  mem_writable Γ (addr_top (N.pos b) sintT) m →
+  Memory.Mem.storev AST.Mint32 ṁ (Vptr b Ptrofs.zero)
+    (Vint (Int.repr z)) = Some ṁ' →
+  int_typed z (sintT: int_type K) →
+  mem_equiv
+    (<[addr_top (N.pos b) sintT:=intV{sintT} z]{Γ}> m)
+    ṁ'.
+Proof.
+  intros ? Hwelltyped; intros.
+  assert (Hvalue_welltyped: (Γ, '{m}) ⊢ intV{sintT} z : sintT%T). {
+    constructor.
+    constructor.
+    assumption.
+  }
+  split.
+  - intros.
+    destruct H.
+    destruct (classic (b0 = b)).
+    + subst.
+      destruct (blocks_equiv0 b). {
+        elim H.
+        eapply mem_writable_alive in H0; try eassumption.
+      }
+      apply block_equiv_alloced with (oz:=Some z).
+      * simpl.
+        simpl in H1.
+        apply Memory.Mem.load_store_same with (1:=H1).
+      * apply Memory.Mem.store_valid_access_1 with (1:=H1).
+        apply Memory.Mem.store_valid_access_3 with (1:=H1).
+      * intro; intros.
+        apply Memory.Mem.perm_store_1 with (1:=H1).
+        apply H4; assumption.
+      * erewrite mem_insert_memenv_of; try eassumption.
+      * erewrite mem_insert_memenv_of; try eassumption.
+      * assert (freeze true (ch2o_val_of (Some z)) = ch2o_val_of (Some z)). reflexivity.
+        rewrite <- H10.
+        eapply mem_lookup_insert; try eassumption.
+        constructor.
+      * eapply mem_insert_writable; try eassumption.
+        tauto.
+      * assumption.
+    + destruct (blocks_equiv0 b0).
+      * apply block_equiv_not_alloced.
+        erewrite mem_insert_memenv_of; eassumption.
+      * apply block_equiv_alloced with (oz:=oz).
+        -- simpl.
+           rewrite Memory.Mem.load_store_other with (1:=H1).
+           ++ assumption.
+           ++ left; assumption.
+        -- apply Memory.Mem.store_valid_access_1 with (1:=H1) (2:=H4).
+        -- intro; intros.
+           apply Memory.Mem.perm_store_1 with (1:=H1).
+           apply H5; assumption.
+        -- erewrite mem_insert_memenv_of; eassumption.
+        -- erewrite mem_insert_memenv_of; try eassumption.
+        -- eapply mem_lookup_insert_disjoint; try eassumption.
+           constructor.
+           simpl.
+           congruence.
+        -- eapply mem_insert_writable; try eassumption.
+           right.
+           constructor.
+           simpl; congruence.
+        -- assumption.
+  - destruct H.
+    intros.
+    rewrite mem_dom_insert.
+    rewrite Memory.Mem.nextblock_store with (1:=H1) in H.
+    auto.
+  - destruct H.
+    eapply mem_insert_valid'; try eassumption.
+Qed.
+
+Inductive env_equiv(ẽ: Csem.env): list AST.ident → list (index * types.type K) → Prop :=
+| env_equiv_nil:
+  env_equiv ẽ [] []
+| env_equiv_cons x ê b ρ:
+  Maps.PTree.get x ẽ = Some (b, tint) →
+  env_equiv ẽ ê ρ →
+  env_equiv ẽ (x::ê) ((Npos b, sintT%T)::ρ)
+.
+
+Lemma env_equiv_lookup:
+  forall ẽ ê ρ,
+  env_equiv ẽ ê ρ →
+  forall i x,
+  ê !! i = Some x →
+  ∃ b, Maps.PTree.get x ẽ = Some (b, tint).
+Proof.
+  induction 1; intros.
+  - discriminate.
+  - destruct i.
+    + simpl in H1; injection H1; clear H1; intros; subst.
+      exists b.
+      assumption.
+    + simpl in H1.
+      apply IHenv_equiv with (1:=H1).
+Qed.
+
+Inductive lrred: Csem.env → kind → expr → Memory.mem → Events.trace → expr → Memory.mem → Prop :=
+| lrred_lred ẽ a ṁ a' ṁ':
+  lred (globalenv p) ẽ a ṁ a' ṁ' →
+  lrred ẽ LV a ṁ Events.E0 a' ṁ'
+| lrred_rred ẽ a ṁ t a' ṁ':
+  rred (globalenv p) a ṁ t a' ṁ' →
+  lrred ẽ RV a ṁ t a' ṁ'
+.
+
+Lemma indexmap_merge_spec A B C (f: option A -> option B -> option C) (t1: indexmap A) (t2: indexmap B) i:
+  f None None = None →
+  merge f t1 t2 !! i = f (t1 !! i) (t2 !! i).
+Proof.
+  intros.
+  destruct t1.
+  destruct t2.
+  destruct i.
+  - simpl.
+    reflexivity.
+  - simpl.
+    destruct Nmap_pos.
+    destruct Nmap_pos0.
+    simpl.
+    unfold pmap.Pmerge.
+    simpl.
+    unfold lookup.
+    unfold pmap.Plookup.
+    simpl.
+    apply pmap.Pmerge_spec.
+    assumption.
+Qed.
+
+Lemma mem_unlock_all_lookup m b v:
+  m !!{Γ} addr_top (N.pos b) sintT = Some v →
+  mem_unlock_all m !!{Γ} addr_top (N.pos b) sintT = Some v.
+Proof.
+  destruct m as [m].
+  simpl.
+  unfold mem_lookup.
+  simpl.
+  unfold cmap_lookup.
+  rewrite option_guard_True. 2:{ constructor. simpl. lia. }
+  simpl.
+  intro.
+  unfold lookup in H.
+  case_eq (indexmap_lookup (N.pos b) m); intros; rewrite H0 in H. 2:{
+    discriminate.
+  }
+  destruct c; try discriminate.
+  simpl in H.
+  destruct (classic (ctree_Forall (λ γb : pbit K, Some Readable ⊆ pbit_kind γb) c)). 2:{
+    rewrite option_guard_False in H; try assumption; discriminate.
+  }
+  rewrite option_guard_True in H; try assumption.
+  injection H; clear H; intros; subst.
+  rewrite indexmap_merge_spec; try reflexivity.
+  rewrite lookup_omap.
+  unfold lookup.
+  rewrite H0.
+  simpl.
+  destruct (classic (natmap.of_bools (pbit_locked <$> ctree_flatten c) ≠ ∅)).
+  - rewrite option_guard_True; try assumption.
+    simpl.
+    rewrite option_guard_True. 2:{
+      rewrite ctree_flatten_merge.
+      apply Forall_zip_with_fst with (1:=H1).
+      apply Forall_forall.
+      intros.
+      destruct x; simpl; try assumption.
+      destruct x0; simpl.
+      simpl in H3.
+      destruct tagged_perm; try assumption.
+      destruct l; try assumption.
+      unfold perm_kind in H3.
+      elim H3.
+    }
+    f_equal.
+    clear H0 H1 H.
+    rewrite natmap.to_of_bools.
+    rewrite resize_all_alt. 2:{
+      unfold fmap.
+      rewrite fmap_length.
+      reflexivity.
+    }
+    apply ctree_ind_alt with (w:=c); intros.
+    + simpl.
+      f_equal.
+      f_equal.
+      induction xs.
+      * reflexivity.
+      * simpl.
+        unfold fmap in IHxs.
+        rewrite IHxs.
+        f_equal; try reflexivity.
+        destruct a.
+        simpl.
+        destruct tagged_perm; try reflexivity.
+        destruct l; reflexivity.
+    + simpl.
+      f_equal.
+      revert H.
+      induction ws; intros; try reflexivity.
+      simpl.
+      inversion H; subst.
+      f_equal.
+      * rewrite <- fmap_take.
+        rewrite take_app.
+        assumption.
+      * rewrite <- fmap_drop.
+        rewrite drop_app.
+        auto.
+    + simpl.
+      f_equal.
+      revert H; induction wxss; intros; simpl. reflexivity.
+      destruct a.
+      simpl.
+      inversion H; clear H; subst.
+      f_equal.
+      * rewrite <- fmap_take.
+        rewrite <- app_assoc.
+        rewrite take_app.
+        assumption.
+      * rewrite <- fmap_drop.
+        rewrite <- fmap_drop.
+        rewrite <- app_assoc.
+        rewrite drop_app.
+        rewrite drop_app.
+        auto.
+    + simpl.
+      f_equal.
+      rewrite <- fmap_take.
+      rewrite take_app.
+      assumption.
+    + simpl.
+      f_equal.
+      induction xs.
+      * reflexivity.
+      * simpl.
+        f_equal.
+        -- destruct a.
+           destruct tagged_perm; try reflexivity.
+           destruct l; reflexivity.
+        -- assumption.
+  - rewrite option_guard_False; try assumption.
+    simpl.
+    rewrite option_guard_True; try assumption.
+    reflexivity.
+Qed.
+
+Lemma mem_writable_unlock_all m b:
+  mem_writable Γ (addr_top (N.pos b) sintT) m →
+  mem_writable Γ (addr_top (N.pos b) sintT) (mem_unlock_all m).
+Proof.
+  unfold mem_writable.
+  intros.
+  destruct H as [w [Hw Hw']].
+  unfold mem_unlock_all.
+  unfold mem_unlock.
+  destruct (mem_locks m) as [Ω].
+  destruct m as [m].
+  simpl.
+  unfold cmap_lookup.
+  rewrite option_guard_True. 2:{ constructor. simpl. lia. }
+  simpl.
+  rewrite indexmap_merge_spec. 2:{ reflexivity. }
+  unfold lookup.
+  simpl in Hw.
+  unfold cmap_lookup in Hw.
+  rewrite option_guard_True in Hw. 2:{ constructor. simpl. lia. }
+  simpl in Hw.
+  unfold lookup in Hw.
+  case_eq (indexmap_lookup (N.pos b) m); intros; rewrite H in Hw. 2:{ discriminate. }
+  destruct c as [|w1 μ]; try discriminate.
+  simpl in Hw.
+  injection Hw; clear Hw; intros; subst.
+  case_eq (indexmap_lookup (N.pos b) Ω); intros.
+  - simpl.
+    eexists; split. reflexivity.
+    rewrite ctree_flatten_merge.
+    apply Forall_zip_with_fst with (1:=Hw').
+    apply Forall_forall; intros.
+    destruct x; simpl; try assumption.
+    destruct x0; try assumption.
+    destruct tagged_perm as [[]|[]]; try assumption.
+    elim H2.
+  - simpl.
+    eexists; split. reflexivity.
+    assumption.
+Qed.
+
+Lemma mem_unlock_all_spec' (m: mem K):
+  mem_unlock_all m =
+    let (m) := m in
+    CMap $ cmap_elem_map (ctree_map pbit_unlock) <$> m.
+Proof.
+  destruct m as [m].
+  unfold mem_unlock_all.
+  simpl.
+  f_equal.
+  apply map_eq; intro i.
+  rewrite indexmap_merge_spec; try reflexivity.
+  rewrite lookup_fmap.
+  rewrite lookup_omap.
+  destruct (m !! i); try reflexivity.
+  destruct c as [|ω μ]; try reflexivity.
+  simpl.
+  destruct (classic (natmap.of_bools (pbit_locked <$> ctree_flatten ω) = ∅)). {
+    rewrite option_guard_False. 2:{
+      tauto.
+    }
+    f_equal.
+    f_equal.
+    Search ctree_map.
+    rewrite ctree_map_id with (P:=λ b, pbit_locked b = false).
+    - reflexivity.
+    - intros.
+      destruct x.
+      destruct tagged_perm; try reflexivity.
+      destruct l.
+      + discriminate.
+      + reflexivity.
+    - apply Forall_lookup_2; intros.
+      case_eq (pbit_locked x); intros; try trivial.
+      assert ((pbit_locked <$> ctree_flatten ω) !! i0 = Some true). {
+        rewrite list_lookup_fmap.
+        rewrite H0.
+        simpl.
+        congruence.
+      }
+      apply natmap.elem_of_of_bools in H2.
+      rewrite H in H2.
+      apply not_elem_of_empty in H2.
+      elim H2.
+  }
+  rewrite option_guard_True; try assumption.
+  f_equal.
+  f_equal.
+  rewrite natmap.to_of_bools.
+  rewrite resize_all_alt. 2:{
+    rewrite fmap_length.
+    reflexivity.
+  }
+  apply ctree_merge_map. {
+    rewrite fmap_length.
+    reflexivity.
+  }
+  clear H.
+  induction (ctree_flatten ω); try reflexivity.
+  simpl.
+  f_equal.
+  - destruct a.
+    destruct tagged_perm; try reflexivity.
+    destruct l0; reflexivity.
+  - apply IHl.
+Qed.
+
+Lemma mem_unlock_all_mem_lock b m:
+  mem_unlock_all (mem_lock Γ (addr_top (N.pos b) sintT) m) = mem_unlock_all m.
+Proof.
+  rewrite mem_unlock_all_spec'.
+  rewrite mem_unlock_all_spec'.
+  destruct m as [m].
+  simpl.
+  f_equal.
+  apply map_eq; intro i.
+  rewrite lookup_fmap.
+  rewrite lookup_fmap.
+  destruct (classic (i = N.pos b)). 2:{
+    rewrite lookup_alter_ne; congruence.
+  }
+  subst.
+  rewrite lookup_alter.
+  destruct (m !! (N.pos b: index)); try reflexivity.
+  simpl.
+  f_equal.
+  destruct c as [|ω μ]; try reflexivity.
+  simpl.
+  f_equal.
+  rewrite <- ctree_map_compose.
+  assert (pbit_unlock (K:=K) ∘ pbit_lock = pbit_unlock). {
+    apply functional_extensionality; intros.
+    destruct x.
+    destruct tagged_perm; try reflexivity.
+    destruct l; reflexivity.
+  }
+  congruence.
+Qed.
+
+Lemma fmap_zip_with {A B C D} (f: C → D) (g: A → B → C) xs ys:
+  f <$> zip_with g xs ys = zip_with (λ x y, f (g x y)) xs ys.
+Proof.
+  revert ys.
+  induction xs; intros; simpl.
+  - reflexivity.
+  - destruct ys.
+    + reflexivity.
+    + simpl.
+      f_equal.
+      apply IHxs.
+Qed.
+
+Lemma ctree_map_ctree_merge {A B C D} (f: C → D) (g: A → B → C) (w: ctree K A) ys:
+  ctree_map f (ctree_merge g w ys) = ctree_merge (λ x y, f (g x y)) w ys.
+Proof.
+  revert ys.
+  apply ctree_ind_alt with (w:=w); intros; simpl.
+  - f_equal.
+    apply fmap_zip_with.
+  - f_equal.
+    revert ys.
+    induction ws; intros; try reflexivity.
+    simpl.
+    inversion H; clear H; subst.
+    f_equal.
+    + apply H2.
+    + apply IHws.
+      apply H3.
+  - f_equal.
+    revert ys.
+    induction wxss; intros; try reflexivity.
+    destruct a.
+    simpl.
+    inversion H; clear H; subst.
+    f_equal.
+    + f_equal.
+      * apply H2.
+      * apply fmap_zip_with.
+    + apply IHwxss.
+      apply H3.
+  - f_equal.
+    + apply H.
+    + apply fmap_zip_with.
+  - f_equal.
+    apply fmap_zip_with.
+Qed.
+
+Lemma mem_unlock_all_mem_unlock Ω (m: mem K):
+  mem_unlock_all (mem_unlock Ω m) = mem_unlock_all m.
+Proof.
+  rewrite !mem_unlock_all_spec'.
+  destruct m as [m].
+  destruct Ω as [Ω HΩ].
+  simpl.
+  f_equal.
+  apply map_eq; intro i.
+  rewrite !lookup_fmap.
+  rewrite indexmap_merge_spec; [|reflexivity].
+  destruct (Ω !! i); try reflexivity.
+  destruct (m !! i); try reflexivity.
+  destruct c as [|w μ]; try reflexivity.
+  simpl.
+  f_equal.
+  f_equal.
+  rewrite ctree_map_ctree_merge.
+  apply ctree_merge_map. {
+    rewrite natmap.to_bools_length.
+    reflexivity.
+  }
+  pose proof (natmap.to_bools_length m0 (Datatypes.length (ctree_flatten w))).
+  revert H.
+  generalize (natmap.to_bools (Datatypes.length (ctree_flatten w)) m0).
+  induction (ctree_flatten w); intros; try reflexivity.
+  simpl.
+  destruct l0; try discriminate.
+  f_equal.
+  - destruct a as [[[]|[]]]; destruct b; try reflexivity.
+  - apply IHl.
+    simpl in H.
+    lia.
+Qed.
+
+Lemma mem_unlock_all_mem_insert b v (m: mem K):
+  mem_unlock_all (<[addr_top (N.pos b) sintT: addr K:=v]{Γ}> m) =
+  <[addr_top (N.pos b) sintT:=v]{Γ}> (mem_unlock_all m).
+Proof.
+  rewrite !mem_unlock_all_spec'.
+  destruct m as [m].
+  simpl.
+  f_equal.
+  apply map_eq; intro i.
+  rewrite !lookup_fmap.
+  destruct (classic (i = N.pos b)). 2:{
+    rewrite !lookup_alter_ne; try congruence.
+    rewrite lookup_fmap.
+    reflexivity.
+  }
+  subst.
+  rewrite !lookup_alter.
+  rewrite lookup_fmap.
+  destruct (m !! (N.pos b: index)); try reflexivity.
+  destruct c as [|ω μ]; try reflexivity.
+  simpl.
+  f_equal.
+  f_equal.
+  rewrite ctree_map_of_val with (g:=perm_unlock). 2:{ intros; reflexivity. }
+  f_equal.
+  rewrite ctree_flatten_map.
+  rewrite <- !list_fmap_compose.
+  reflexivity.
+Qed.
+
+Lemma mem_unlock_all_mem_alloc o μ γ v (m: mem K):
+  perm_unlock γ = γ →
+  mem_unlock_all (mem_alloc Γ o μ γ v m) =
+  mem_alloc Γ o μ γ v (mem_unlock_all m).
+Proof.
+  intros ?.
+  rewrite !mem_unlock_all_spec'.
+  destruct m as [m].
+  simpl.
+  f_equal.
+  rewrite fmap_insert.
+  f_equal.
+  simpl.
+  f_equal.
+  rewrite ctree_map_of_val with (g:=perm_unlock). 2:{ intros; reflexivity. }
+  f_equal.
+  rewrite fmap_replicate.
+  f_equal.
+  assumption.
+Qed.
+
+Lemma mem_unlock_all_mem_free o (m: mem K):
+  mem_unlock_all (mem_free o m) = mem_free o (mem_unlock_all m).
+Proof.
+  destruct m as [m].
+  rewrite !mem_unlock_all_spec'.
+  simpl.
+  f_equal.
+  apply map_eq; intro i.
+  rewrite !lookup_fmap.
+  destruct (classic (o = i)).
+  - subst.
+    rewrite lookup_alter.
+    rewrite lookup_alter.
+    rewrite lookup_fmap.
+    destruct (m !! i) as [[|w μ]|]; try reflexivity.
+    simpl.
+    rewrite ctree_map_type_of.
+    reflexivity.
+  - rewrite !lookup_alter_ne with (1:=H).
+    rewrite lookup_fmap.
+    reflexivity.
+Qed.
+
+Lemma dom_mem_unlock_all (m: mem K): dom indexset (mem_unlock_all m) = dom indexset m.
+Proof.
+  rewrite mem_unlock_all_spec'.
+  destruct m as [m].
+  simpl.
+  apply dom_fmap_L.
+Qed.
+
+Lemma memenv_of_mem_unlock_all (m: mem K): '{mem_unlock_all m} = '{m}.
+Proof.
+  rewrite mem_unlock_all_spec'.
+  destruct m as [m].
+  simpl.
+  apply map_eq; intro i.
+  rewrite !lookup_fmap.
+  destruct (m !! i); try reflexivity.
+  destruct c as [|w μ]; simpl; try reflexivity.
+  rewrite ctree_map_type_of.
+  reflexivity.
+Qed.
+
+Lemma lrred_safe e ė θ:
+  expr_equiv e ė θ →
+  ∀ C K_ K_' a ẽ ṁ t a' ṁ' ρ m,
+  context K_ K_' C →
   ė = C a →
-  rred ẽ a ṁ t a' ṁ' →
-  ∃ (E: ectx K) e1 e2,
+  lrred ẽ K_ a ṁ t a' ṁ' →
+  mem_equiv (mem_unlock_all m) ṁ →
+  env_equiv ẽ ê ρ →
+  ∀(Hsafe: ∀ (E: ectx K) e1, e = subst E e1 → is_redex e1 → Γ \ ρ ⊢ₕ safe e1, m),
+  ∃ (E: ectx K) e1 e2 m',
   e = subst E e1 ∧
-  Γ \ ρ ⊢ₕ e1, m ⇒ e2, m ∧
-  expr_equiv (subst E e2) (C a') ∧
-  ṁ' = ṁ.
+  Γ \ ρ ⊢ₕ e1, m ⇒ e2, m' ∧
+  expr_equiv (subst E e2) (C a') θ ∧
+  mem_equiv (mem_unlock_all m') ṁ' ∧
+  '{m'} = '{m}.
 Proof.
 induction 1; intros.
 - inversion H0; clear H0; subst; try discriminate.
   subst.
-  inversion H2.
-- inversion H1; clear H1; subst; try discriminate.
+  inversion H2; clear H2; subst; inversion H0.
+- rename H4 into Hmem_equiv.
+  rename H5 into Menv_equiv.
+  inversion H1; clear H1; subst; try discriminate.
   + subst.
-    inversion H3; clear H3; subst.
-    inversion H; clear H; subst.
-    inversion H0; clear H0; subst.
+    inversion H3; clear H3; subst; inversion H1; clear H1; subst.
+    inversion H; clear H; subst;
+    inversion H0; clear H0; subst; try discriminate.
     simpl in H10.
     unfold sem_div in H10.
     unfold sem_binarith in H10.
@@ -406,7 +1036,7 @@ induction 1; intros.
     destruct H.
     subst.
     exists [].
-    eexists; eexists.
+    eexists; eexists; eexists.
     simpl; split; [reflexivity|].
     split. {
       constructor. constructor.
@@ -414,17 +1044,20 @@ induction 1; intros.
       -- apply H.
     }
     split. {
-      rewrite (right_id_L _ (∪)).
       unfold Int.divs.
       rewrite Int.signed_repr. 2:{ apply int_typed_limits; assumption. }
       rewrite Int.signed_repr. 2:{ apply int_typed_limits; assumption. }
       constructor.
       assumption.
     }
-    reflexivity.
+    split. assumption. reflexivity.
   + injection H2; clear H2; intros; subst.
-    destruct (IHexpr_equiv1 C0 a ẽ ṁ t a' ṁ' ρ m H4) as [E [e5 [e6 [? [? ?]]]]]; try trivial.
-    exists (E ++ [CBinOpL (ArithOp DivOp) e2])%E; eexists; eexists.
+    destruct (IHexpr_equiv1 C0 K_ RV a ẽ ṁ t a' ṁ' ρ m H4) as [E [e5 [e6 [m' [? [? ?]]]]]]; try trivial. {
+      intros; subst.
+      apply Hsafe with (E0:=E++[CBinOpL (ArithOp DivOp) e2]) (2:=H2).
+      rewrite subst_snoc; reflexivity.
+    }
+    exists (E ++ [CBinOpL (ArithOp DivOp) e2])%E; eexists; eexists; eexists.
     rewrite subst_snoc.
     rewrite subst_snoc.
     simpl.
@@ -434,23 +1067,227 @@ induction 1; intros.
     split. { constructor; tauto. }
     destruct H5; congruence.
   + injection H2; clear H2; intros; subst.
-    destruct (IHexpr_equiv2 C0 a ẽ ṁ t a' ṁ' ρ m H4) as [E [e5 [e6 [? [? [? Hṁ']]]]]]; try trivial.
-    exists (E ++ [CBinOpR (ArithOp DivOp) e1])%E; eexists; eexists.
+    destruct (IHexpr_equiv2 C0 K_ RV a ẽ ṁ t a' ṁ' ρ m H4) as [E [e5 [e6 [m' [? [? [? Hṁ']]]]]]]; try trivial. {
+      intros; subst.
+      apply Hsafe with (E0:=E++[CBinOpR (ArithOp DivOp) e1]) (2:=H2).
+      rewrite subst_snoc; reflexivity.
+    }
+    exists (E ++ [CBinOpR (ArithOp DivOp) e1])%E; eexists; eexists; eexists.
     rewrite subst_snoc.
     rewrite subst_snoc.
     simpl.
     rewrite H1.
     split; try trivial.
     split. { apply H2. }
-    split. { constructor; assumption. }
+    split. { constructor; tauto. }
+    destruct H5; congruence.
+- (* var i *)
+  inversion H0; clear H0; subst; try discriminate.
+  subst.
+  inversion H2; clear H2; subst; inversion H0; clear H0; subst. 2:{
+    apply False_ind.
+    clear Hsafe.
+    revert H4 i H.
+    induction 1; intros.
+    - discriminate.
+    - destruct i.
+      + simpl in H0.
+        injection H0; clear H0; intros; subst.
+        congruence.
+      + simpl in H0.
+        eapply IHenv_equiv; eassumption.
+  }
+  exists [].
+  exists (var i)%E.
+  exists (%(Ptr (addr_top (Npos b) sintT)))%E.
+  exists m.
+  split. { reflexivity. }
+  split. {
+    constructor.
+    clear Hsafe.
+    revert H4 i H.
+    induction 1; intros.
+    - discriminate.
+    - destruct i.
+      + simpl in H0.
+        injection H0; clear H0; intros; subst.
+        assert (b0 = b). congruence.
+        subst.
+        reflexivity.
+      + simpl in *.
+        apply IHenv_equiv; assumption.
+  }
+  split. {
+    constructor.
+  }
+  split. assumption. reflexivity.
+- (* loc *)
+  inversion H; clear H; subst; try discriminate.
+  subst.
+  inversion H1; clear H1; subst; inversion H; clear H; subst.
+- (* load *)
+  inversion H0; clear H0; subst; try discriminate.
+  + subst.
+    inversion H2; clear H2; subst; inversion H0; clear H0; subst.
+    inversion H; clear H; subst.
+    inversion H9; clear H9; subst; try discriminate.
+    simpl in H.
+    injection H; clear H; intros; subst.
+    pose proof (blocks_equiv _ _ H3 b).
+    assert (Hsafe': Γ \ ρ ⊢ₕ safe (load (% Ptr (addr_top (N.pos b) sintT))), m). {
+      apply Hsafe with (E:=[]); try reflexivity.
+      repeat constructor.
+    }
+    inversion Hsafe'; clear Hsafe'; subst.
+    inversion H2; clear H2; subst; try congruence.
+    pose proof H10.
+    apply mem_lookup_index_alive in H2.
+    rewrite <- memenv_of_mem_unlock_all in H2.
+    inversion H; clear H; subst; try tauto.
+    assert (v = compcert_val_of oz). congruence. subst.
+    exists []; eexists; eexists; exists m.
+    split. { reflexivity. }
+    split. {
+      assert (m = mem_force Γ (addr_top (N.pos b) sintT) m). {
+        unfold mem_force.
+        simpl.
+        unfold cmap_alter_ref.
+        destruct m.
+        simpl.
+        rewrite alter_id.
+        - reflexivity.
+        - intros.
+          unfold cmap_elem_map.
+          destruct x; reflexivity.
+      }
+      rewrite H at 2.
+      constructor.
+      eassumption.
+    }
+    split. {
+      apply mem_unlock_all_lookup in H10.
+      rewrite H10 in H11.
+      injection H11; clear H11; intros; subst.
+      destruct oz; constructor.
+      assumption.
+    }
+    split. assumption. reflexivity.
+  + injection H1; clear H1; intros; subst.
+    destruct (IHexpr_equiv _ _ _ _ _ _ _ _ _ _ _ H5 eq_refl H2 H3 H4) as [E [e1 [e2 [m' [? [? [? ?]]]]]]]. {
+      intros; subst.
+      apply Hsafe with (E0:=E++[CLoad]) (2:=H1).
+      rewrite subst_snoc; reflexivity.
+    }
+    subst.
+    exists (E ++ [CLoad]); eexists; eexists; eexists.
+    rewrite ! subst_snoc; simpl.
+    split. { reflexivity. }
+    split. { eassumption. }
+    split. {
+      simpl.
+      constructor; assumption.
+    }
     assumption.
+- (* indetV *)
+  inversion H; clear H; subst; try discriminate.
+  subst.
+  inversion H1; clear H1; subst; inversion H; clear H; subst.
+- (* assign *)
+  inversion H1; clear H1; subst; try discriminate.
+  + subst.
+    inversion H3; clear H3; subst; inversion H1; clear H1; subst.
+    inversion H; clear H; subst.
+    inversion H0; clear H0; subst.
+    * rewrite sem_cast_int in H11.
+      injection H11; clear H11; subst.
+      inversion H12; clear H12; subst; try discriminate.
+      intros; subst.
+      simpl in H.
+      injection H; clear H; intros; subst.
+      lapply (Hsafe [] _ eq_refl). 2:{ repeat constructor. }
+      intros.
+      inversion H; clear H; subst.
+      inversion H3; clear H3; subst.
+      exists []; eexists; eexists; eexists.
+      split. { reflexivity. }
+      split. {
+        constructor; eassumption.
+      }
+      inversion H14; clear H14.
+      simpl in H3.
+      erewrite int_cast_self in H3; try assumption.
+      subst.
+      split. {
+        simpl.
+        constructor.
+        assumption.
+      }
+      rewrite mem_unlock_all_mem_lock.
+      rewrite mem_unlock_all_mem_insert.
+      inversion H4; subst.
+      pose proof H13.
+      apply mem_writable_unlock_all in H3.
+      eapply mem_writable_alive with (Δ:='{mem_unlock_all m}) in H3; try eassumption.
+      destruct (blocks_equiv0 b); try tauto.
+      split. {
+        eapply mem_equiv_insert; try eassumption.
+      }
+      rewrite <- memenv_of_mem_unlock_all.
+      rewrite mem_unlock_all_mem_lock.
+      rewrite mem_unlock_all_mem_insert.
+      rewrite <- memenv_of_mem_unlock_all with (m:=m).
+      eapply mem_insert_memenv_of; try eassumption.
+      constructor.
+      constructor.
+      assumption.
+    * lapply (Hsafe [] _ eq_refl). 2:{ repeat constructor. }
+      intros.
+      inversion H; clear H; subst.
+      inversion H0; clear H0; subst.
+      inversion H13; clear H13; subst.
+      inversion H; clear H; subst.
+      discriminate.
+  + injection H2; clear H2; intros; subst.
+    destruct (IHexpr_equiv1 _ _ _ _ _ _ _ _ _ _ _ H6 eq_refl H3 H4 H5) as [E [e1' [e2' [m' [? [? [? ?]]]]]]]. {
+      intros; subst.
+      apply Hsafe with (E0:=E++[CAssignL Assign e2]) (2:=H2).
+      rewrite subst_snoc; reflexivity.
+    }
+    subst.
+    exists (E ++ [CAssignL Assign e2]); eexists; eexists; eexists.
+    rewrite ! subst_snoc; simpl.
+    split. { reflexivity. }
+    split. { eassumption. }
+    split. {
+      simpl.
+      constructor; assumption.
+    }
+    assumption.
+  + injection H2; clear H2; intros; subst.
+    destruct (IHexpr_equiv2 _ _ _ _ _ _ _ _ _ _ _ H6 eq_refl H3 H4 H5) as [E [e1' [e2' [m' [? [? [? ?]]]]]]]. {
+      intros; subst.
+      apply Hsafe with (E0:=E++[CAssignR Assign e1]) (2:=H2).
+      rewrite subst_snoc; reflexivity.
+    }
+    subst.
+    exists (E ++ [CAssignR Assign e1]); eexists; eexists; eexists.
+    rewrite ! subst_snoc; simpl.
+    split. { reflexivity. }
+    split. { eassumption. }
+    split. {
+      simpl.
+      constructor; assumption.
+    }
+    assumption.
+  Unshelve.
+  exact (IntEnvSpec_instance_0 A).
 Qed.
 
-Lemma expr_equiv_no_call e ė:
-  expr_equiv e ė →
-  ∀ a m fd vargs ty C,
+Lemma expr_equiv_no_call e ė θ:
+  expr_equiv e ė θ →
+  ∀ a m fd vargs ty K C,
   callred (globalenv p) a m fd vargs ty →
-  context RV RV C →
+  context RV K C →
   ė ≠ C a.
 Proof.
 induction 1; intros.
@@ -466,54 +1303,114 @@ induction 1; intros.
   + intro.
     injection H4; clear H4; intros; subst.
     apply IHexpr_equiv2 with (1:=H1) (2:=H3) (3:=eq_refl).
+- inversion H1; subst; try discriminate.
+  intro; subst.
+  inversion H0.
+- inversion H0; subst; try discriminate.
+  intro; subst.
+  inversion H.
+- inversion H1; subst; try discriminate.
+  + intro; subst.
+    inversion H0.
+  + intro.
+    injection H3; clear H3; intros; subst.
+    apply IHexpr_equiv with (1:=H0) (2:=H2) (3:=eq_refl).
+- inversion H0; subst; try discriminate.
+  intro; subst.
+  inversion H.
+- inversion H2; subst; try discriminate.
+  + intro.
+    subst.
+    inversion H1.
+  + intro.
+    injection H4; clear H4; intros; subst.
+    apply IHexpr_equiv1 with (1:=H1) (2:=H3).
+    reflexivity.
+  + intro.
+    injection H4; clear H4; intros; subst.
+    apply IHexpr_equiv2 with (1:=H1) (2:=H3).
+    reflexivity.
 Qed.
 
-Lemma expr_equiv_imm_safe_rred e ė:
-  expr_equiv e ė →
-  ∀ ρ m,
+Definition kind_of_type(θ: type_): kind :=
+  match θ with
+    Int => RV
+  | Loc => LV
+  end.
+
+Lemma expr_equiv_imm_safe e ė θ:
+  expr_equiv e ė θ →
+  ∀ m ṁ ẽ ρ,
+  mem_equiv (mem_unlock_all m) ṁ →
+  env_equiv ẽ ê ρ →
   (∀ (E: ectx K) e1, e = subst E e1 → is_redex e1 → Γ \ ρ ⊢ₕ safe e1, m) →
-  (∃ v ty, ė = Eval v ty) ∨
-  ∀ ṁ,
-  ∃ C a t a',
-  context RV RV C ∧
-  ė = C a ∧ rred (globalenv p) a ṁ t a' ṁ.
+  imm_safe (globalenv p) ẽ (kind_of_type θ) ė ṁ.
 Proof.
 induction 1; intros.
-- left. eexists; eexists; reflexivity.
-- right.
-  intros.
-  destruct (IHexpr_equiv1 ρ m). {
+- apply imm_safe_val.
+- assert (imm_safe (globalenv p) ẽ RV ė1 ṁ). {
+    eapply IHexpr_equiv1; try eassumption.
     intros.
-    apply H1 with (2:=H3) (E:=(E++[CBinOpL (ArithOp DivOp) e2])).
+    subst.
+    apply (H3 (E++[CBinOpL (ArithOp DivOp) e2])); try assumption.
+    simpl.
     rewrite subst_snoc.
-    rewrite H2.
     reflexivity.
   }
-  + destruct (IHexpr_equiv2 ρ m). {
-      intros.
-      apply H1 with (2:=H4) (E:=(E++[CBinOpR (ArithOp DivOp) e1])).
+  inversion H4; clear H4; subst.
+  + assert (imm_safe (globalenv p) ẽ RV ė2 ṁ). {
+      eapply IHexpr_equiv2; try eassumption.
+      intros; subst.
+      apply (H3 (E++[CBinOpR (ArithOp DivOp) e1])); try assumption.
       rewrite subst_snoc.
-      rewrite H3.
       reflexivity.
     }
-    * destruct H2 as [v1 [ty1 ?]].
-      destruct H3 as [v2 [ty2 ?]].
-      subst.
-      inversion H; clear H; subst.
-      inversion H0; clear H0; subst.
-      eexists; eexists; eexists; eexists.
-      split. { apply ctx_top. }
-      split. { simpl; reflexivity. }
+    inversion H4; clear H4; subst.
+    * inversion H; clear H; subst. 2:{
+        inversion H0; clear H0; subst.
+        -- lapply (H3 [] _ eq_refl). 2:{
+             constructor.
+             constructor.
+             constructor.
+           }
+           intros.
+           inversion H; clear H; subst.
+           inversion H0; clear H0; subst.
+           inversion H12; clear H12; subst.
+        -- lapply (H3 [] _ eq_refl). 2:{
+             constructor.
+             constructor.
+             constructor.
+           }
+           intros.
+           inversion H; clear H; subst.
+           inversion H0; clear H0; subst.
+           inversion H11; clear H11; subst.
+      }
+      inversion H0; clear H0; subst. 2:{
+        lapply (H3 [] _ eq_refl). 2:{
+           constructor.
+           constructor.
+           constructor.
+         }
+         intros.
+         inversion H; clear H; subst.
+         inversion H0; clear H0; subst.
+         inversion H12; clear H12; subst.
+      }
+      eapply imm_safe_rred with (C:=λ x, x). 2:{
+        apply ctx_top.
+      }
       constructor.
       simpl.
-      assert (Γ \ ρ ⊢ₕ safe (# intV{sintT} z / # intV{sintT} z0)%E, m). {
-        apply H1 with (E:=[]).
+      assert (Γ \ ρ ⊢ₕ safe (#{Ω} intV{sintT} z / #{Ω0} intV{sintT} z0)%E, m). {
+        apply H3 with (E:=[]).
         - reflexivity.
         - constructor; constructor.
       }
       inversion H; clear H; subst.
       inversion H0; clear H0; subst.
-      inversion H11; clear H11; subst.
+      inversion H13; clear H13; subst.
       assert (z0 ≠ 0)%Z. { apply H. }
       assert (int_typed (z ÷ z0) (sintT%IT: int_type K)). { apply H0. }
       clear H H0.
@@ -547,7 +1444,7 @@ induction 1; intros.
         destruct (Coqlib.zeq z (-2147483648)). {
           destruct (Coqlib.zeq z0 (-1)). {
             subst.
-            destruct H5.
+            destruct H7.
             rewrite int_upper_sintT in H0.
             discriminate.
           }
@@ -557,196 +1454,324 @@ induction 1; intros.
       }
       rewrite H.
       reflexivity.
-    * destruct (H3 ṁ) as [C [a [t [a' [HC [Hė2 Hrred]]]]]].
-      subst.
-      exists (λ x, Ebinop Odiv ė1 (C x) tint).
-      eexists; eexists; eexists.
-      split. {
-        constructor.
-        assumption.
+    * eapply imm_safe_lred with (C:=λ x, Ebinop Odiv (Eval v ty) (C x) tint). 2:{
+        apply ctx_binop_right; assumption.
       }
-      split. {
-        reflexivity.
+      eassumption.
+    * eapply imm_safe_rred with (C:=λ x, Ebinop Odiv (Eval v ty) (C x) tint). 2:{
+        apply ctx_binop_right; assumption.
       }
-      eapply Hrred.
-  + destruct (H2 ṁ) as [C [a [t [a' [HC [Hė1 Hrred]]]]]].
-    subst.
-    exists (λ x, Ebinop Odiv (C x) ė2 tint).
-    eexists; eexists; eexists.
-    split. {
-      constructor.
-      assumption.
+      eassumption.
+    * eelim (expr_equiv_no_call _ _ _ H0); try eassumption.
+      reflexivity.
+  + eapply imm_safe_lred with (C:=λ x, Ebinop Odiv (C x) ė2 tint). 2:{
+      apply ctx_binop_left; assumption.
     }
-    split. {
+    eassumption.
+  + eapply imm_safe_rred with (C:=λ x, Ebinop Odiv (C x) ė2 tint). 2:{
+      apply ctx_binop_left; assumption.
+    }
+    eassumption.
+  + eelim (expr_equiv_no_call _ _ _ H); try eassumption.
+    reflexivity.
+- destruct (env_equiv_lookup _ _ _ H1 _ _ H).
+  eapply imm_safe_lred with (C:=λ x, x). 2:{ apply ctx_top. }
+  constructor.
+  eassumption.
+- apply imm_safe_loc.
+- assert (imm_safe (globalenv p) ẽ LV ė ṁ). {
+    eapply IHexpr_equiv; try eassumption.
+    intros; subst.
+    apply H2 with (E0:=E++[CLoad]); try assumption.
+    rewrite subst_snoc.
+    reflexivity.
+  }
+  inversion H3; clear H3; subst.
+  + inversion H; clear H; subst.
+    lapply (H2 [] _ eq_refl). 2:{ constructor. constructor. }
+    intros.
+    inversion H; clear H; subst.
+    inversion H3; clear H3; subst.
+    pose proof H8.
+    apply mem_lookup_index_alive in H.
+    rewrite <- memenv_of_mem_unlock_all in H.
+    destruct (blocks_equiv _ _ H0 b); try tauto.
+    eapply imm_safe_rred with (C:=λ x, x). 2:{ apply ctx_top. }
+    constructor.
+    eapply deref_loc_value; try reflexivity.
+    apply H3.
+  + eapply imm_safe_lred with (C:=λ x, Evalof (C x) tint). 2:{ constructor. assumption. }
+    eassumption.
+  + eapply imm_safe_rred with (C:=λ x, Evalof (C x) tint). 2:{ constructor. assumption. }
+    eassumption.
+  + eelim (expr_equiv_no_call _ _ _ H); eauto.
+- apply imm_safe_val.
+- assert (imm_safe (globalenv p) ẽ LV ė1 ṁ). {
+    eapply IHexpr_equiv1; try eassumption.
+    intros; subst.
+    apply H3 with (E0:=E++[CAssignL Assign e2]); try assumption.
+    rewrite subst_snoc.
+    reflexivity.
+  }
+  inversion H4; clear H4; subst.
+  + assert (imm_safe (globalenv p) ẽ RV ė2 ṁ). {
+      eapply IHexpr_equiv2; try eassumption.
+      intros; subst.
+      apply H3 with (E0:=E++[CAssignR Assign e1]); try assumption.
+      rewrite subst_snoc.
       reflexivity.
     }
-    eapply Hrred.
+    inversion H4; clear H4; subst.
+    * inversion H; clear H; subst.
+      inversion H0; clear H0; subst.
+      -- lapply (H3 [] _ eq_refl). 2:{ constructor. constructor. constructor. }
+         intros.
+         inversion H; clear H; subst.
+         inversion H0; clear H0; subst.
+         pose proof H12.
+         destruct H1.
+         apply mem_writable_unlock_all in H.
+         eapply mem_writable_alive in H; try eassumption.
+         destruct (blocks_equiv0 b); try tauto.
+         edestruct Memory.Mem.valid_access_store with (1:=H1).
+         eapply imm_safe_rred with (C:=λ x, x). 2:{ apply ctx_top. }
+         econstructor; try reflexivity.
+         econstructor; try reflexivity.
+         apply e.
+      -- lapply (H3 [] _ eq_refl). 2:{ constructor. constructor. constructor. }
+         intros.
+         inversion H; clear H; subst.
+         inversion H0; clear H0; subst.
+         inversion H12; clear H12; subst.
+         inversion H; clear H; subst.
+         discriminate.
+    * eapply imm_safe_lred with (C:=λ x, Eassign (Eloc b ofs ty) (C x) tint). 2:{ constructor. assumption. }
+      eassumption.
+    * eapply imm_safe_rred with (C:=λ x, Eassign (Eloc b ofs ty) (C x) tint). 2:{ constructor. assumption. }
+      eassumption.
+    * eelim (expr_equiv_no_call _ _ _ H0); eauto.
+  + eapply imm_safe_lred with (C:=λ x, Eassign (C x) ė2 tint). 2:{ constructor; assumption. }
+    eassumption.
+  + eapply imm_safe_rred with (C:=λ x, Eassign (C x) ė2 tint). 2:{ constructor; assumption. }
+    eassumption.
+  + eelim (expr_equiv_no_call _ _ _ H); eauto.
 Qed.
 
-Lemma expr_equiv_imm_safe e ė:
-  expr_equiv e ė →
-  ∀ K_ C a ρ m ẽ ṁ,
-  context K_ RV C →
+Lemma expr_equiv_subexpr_imm_safe:
+  ∀ K1 K2 C,
+  context K1 K2 C →
+  ∀ e ė θ,
+  expr_equiv e ė θ →
+  K2 = kind_of_type θ →
+  ∀ m ṁ ẽ ρ a,
+  mem_equiv (mem_unlock_all m) ṁ →
+  env_equiv ẽ ê ρ →
   ė = C a →
   (∀ (E: ectx K) e1, e = subst E e1 → is_redex e1 → Γ \ ρ ⊢ₕ safe e1, m) →
-  imm_safe (globalenv p) ẽ K_ a ṁ.
+  imm_safe (globalenv p) ẽ K1 a ṁ.
 Proof.
-induction 1; intros.
-- inversion H0; clear H0; subst; try discriminate.
-  subst.
-  constructor.
-- inversion H1; clear H1; subst; try discriminate.
-  + subst.
-    edestruct (expr_equiv_imm_safe_rred (e1 / e2) (Ebinop Odiv ė1 ė2 tint))%E. {
-      constructor; assumption.
-    } {
-      eassumption.
-    }
-    * destruct H1 as [? [? ?]]; discriminate.
-    * destruct (H1 ṁ) as [C [a [t [a' [HC [Hė Hrred]]]]]].
-      rewrite Hė.
-      eapply imm_safe_rred with (C:=C) (e0:=a); eassumption.
-  + injection H2; clear H2; intros; subst.
-    eapply IHexpr_equiv1; try eassumption.
-    * reflexivity.
-    * intros.
-      eapply H3 with (E:=E++[CBinOpL (ArithOp DivOp) e2]); try assumption.
-      rewrite subst_snoc.
-      simpl.
-      congruence.
-  + injection H2; clear H2; intros; subst.
-    eapply IHexpr_equiv2; try eassumption.
-    * reflexivity.
-    * intros.
-      eapply H3 with (E:=E++[CBinOpR (ArithOp DivOp) e1]); try assumption.
-      rewrite subst_snoc.
-      simpl.
-      congruence.
+  induction 1; intros; subst; try (eapply expr_equiv_imm_safe; eassumption);
+  inversion H0; clear H0; subst.
+  - eapply IHcontext; eauto.
+    intros; subst.
+    eapply H5 with (E0:=E++[CLoad]) (2:=H4).
+    rewrite subst_snoc; reflexivity.
+  - eapply IHcontext with (1:=H11); eauto.
+    intros; subst.
+    eapply H5 with (E0:=E++[CBinOpL (ArithOp DivOp) e0]) (2:=H4).
+    rewrite subst_snoc; reflexivity.
+  - eapply IHcontext with (1:=H12); eauto.
+    intros; subst.
+    eapply H5 with (E0:=E++[CBinOpR (ArithOp DivOp) e0]) (2:=H4).
+    rewrite subst_snoc; reflexivity.
+  - eapply IHcontext with (1:=H10); eauto.
+    intros; subst.
+    eapply H5 with (E0:=E++[CAssignL Assign e0]); eauto.
+    rewrite subst_snoc; reflexivity.
+  - eapply IHcontext with (1:=H11); eauto.
+    intros; subst.
+    eapply H5 with (E0:=E++[CAssignR Assign e0]); eauto.
+    rewrite subst_snoc; reflexivity.
 Qed.
 
-Lemma eval_soundness Q n e ė k ḳ m ṁ f:
-  expr_equiv e ė →
+Lemma ch2o_safe_state_subexpr_safe Q k e m:
   ch2o_safe_state Γ δ Q (State k (Expr e) m) →
-  (∀ z n',
-   n' ≤ n →
-   int_typed z (sintT: int_type K) →
-   ch2o_safe_state Γ δ Q (State k (Expr (# intV{sintT} z)) m) →
-   compcertc_safe_state_n Q p n' (ExprState f (Eval (Vint (Int.repr z)) (Tint I32 Signed noattr)) ḳ empty_env ṁ)) →
-  compcertc_safe_state_n Q p n (ExprState f ė ḳ empty_env ṁ).
+  ∀ (E : ectx K) (e1 : expressions.expr K),
+  e = subst E e1 → is_redex e1 → Γ \ locals k ⊢ₕ safe e1, m.
 Proof.
-revert e ė.
+  intros.
+  destruct (classic (Γ \ locals k ⊢ₕ safe e1, m)); try assumption.
+  edestruct H.
+  - eapply rtc_l.
+    + rewrite H0.
+      eapply cstep_expr_undef; eassumption.
+    + apply rtc_refl.
+  - inversion H3.
+  - destruct H3.
+    inversion H3.
+Qed.
+
+Lemma eval_soundness Q n e ė k ḳ m ṁ ẽ f:
+  expr_equiv e ė Int →
+  mem_equiv (mem_unlock_all m) ṁ →
+  env_equiv ẽ ê (locals k) →
+  ∀(Hlocals_alive: Forall (λ iτ, index_alive '{m} (iτ.1)) (locals k)),
+  ch2o_safe_state Γ δ Q (State k (Expr e) m) →
+  (∀ n',
+   n' ≤ n →
+   ∀ Ω ν v m' ṁ',
+   ∀(Hlocals_alive: Forall (λ iτ, index_alive '{m'} (iτ.1)) (locals k)),
+   ch2o_safe_state Γ δ Q (State k (Expr (%#{ Ω } ν)) m') →
+   expr_equiv (%#{ Ω } ν) v Int →
+   mem_equiv (mem_unlock_all m') ṁ' →
+   compcertc_safe_state_n Q p n' (ExprState f v ḳ ẽ ṁ')) →
+  compcertc_safe_state_n Q p n (ExprState f ė ḳ ẽ ṁ).
+Proof.
+revert e ė m ṁ.
 apply well_founded_induction with (1:=lt_wf) (a:=n).
 clear n.
 intros n IH.
-intros.
+intros e ė m ṁ ? Hmem_equiv Henv_equiv; intros.
 intros t s HstarN.
 inversion HstarN; subst.
 - (* refl *)
-  destruct (compcertc_expr_never_stuck f ė ḳ empty_env ṁ).
+  destruct (compcertc_expr_never_stuck f ė ḳ ẽ ṁ).
   + destruct H2 as [v [ty H2]].
     subst.
     inversion H; clear H; subst.
-    unfold compcertc_safe_state_n in H1.
-    eapply H1 with (n':=0) (trace:=[]); try eauto.
+    * unfold compcertc_safe_state_n in H1.
+      eapply H1 with (n':=0) (trace:=[]); try eauto.
+      constructor.
+      assumption.
+    * unfold compcertc_safe_state_n in H1.
+      eapply H1 with (n':=0) (trace:=[]); try eauto.
+      constructor.
   + tauto.
 - case_eq (match ė with Eval _ _ => true | _ => false end); intros. {
     inversion H; clear H; subst; try discriminate.
-    unfold compcertc_safe_state_n in H1.
-    eapply H1 with (n':=S n0) (4:=HstarN); try eauto.
+    - unfold compcertc_safe_state_n in H1.
+      eapply H1 with (n':=S n0) (6:=HstarN); try eauto.
+      constructor.
+      assumption.
+    - unfold compcertc_safe_state_n in H1.
+      eapply H1 with (n':=S n0) (6:=HstarN); try eauto.
+      constructor.
   }
   destruct H2. 2:{
     inversion H2; subst; discriminate.
   }
   inversion H2; clear H2; subst.
-  + (* step_lred *)
-    eapply expr_equiv_no_LV_context in H; [elim H; reflexivity | assumption].
-  + (* step_rred *)
-    edestruct (rred_safe _ _ H) as [E [e1 [e2 [He1 [He1e2 [Hee' Hṁ']]]]]]; try (eassumption || reflexivity).
+  + (* step_Lred *)
+    rename m' into ṁ'.
+    edestruct (lrred_safe _ _ _ H) as [E [e1 [e2 [m' [He1 [He1e2 [Hee' [Hṁ' Hlocals_alive']]]]]]]]; try (eassumption || reflexivity). {
+      apply lrred_lred.
+      eassumption.
+    } { apply ch2o_safe_state_subexpr_safe with (1:=H0). }
     unfold compcertc_safe_state_n in IH.
     subst.
-    eapply IH with (2:=Hee') (5:=H3).
+    eapply IH with (2:=Hee') (8:=H3); try eassumption.
     * lia.
+    * rewrite Hlocals_alive'; assumption.
     * intro S'.
       intro HS'.
       apply H0.
       eapply rtc_l; try eassumption.
-      assert (∀ e, cast{sintT%T} (subst E e) = subst (E ++ [CCast (sintT%T)]) e)%E. {
-        intros; rewrite subst_snoc.
-        reflexivity.
-      }
       apply cstep_expr_head.
       apply He1e2.
-    * intros z n' Hn'.
-      apply (H1 z n'); lia.
+    * intros n' Hn'.
+      apply (H1 n'); lia.
+  + (* step_rred *)
+    rename m' into ṁ'.
+    edestruct (lrred_safe _ _ _ H) as [E [e1 [e2 [m' [He1 [He1e2 [Hee' [Hṁ' Hlocals_alive']]]]]]]]; try (eassumption || reflexivity). {
+      apply lrred_rred; eassumption.
+    } { apply ch2o_safe_state_subexpr_safe with (1:=H0). }
+    unfold compcertc_safe_state_n in IH.
+    subst.
+    eapply IH with (2:=Hee') (8:=H3); try eassumption.
+    * lia.
+    * rewrite Hlocals_alive'; assumption.
+    * intro S'.
+      intro HS'.
+      apply H0.
+      eapply rtc_l; try eassumption.
+      apply cstep_expr_head.
+      apply He1e2.
+    * intros n' Hn'.
+      apply (H1 n'); lia.
   + (* step_call *)
     apply expr_equiv_no_call with (2:=H12) (3:=H13) in H.
     elim H; reflexivity.
-  + elim H13.
-    eapply expr_equiv_imm_safe with (1:=H) (2:=H12). { reflexivity. }
-    intros.
-    destruct (classic (Γ \ locals k ⊢ₕ safe e1, m)); try eassumption.
-    destruct (H0 (State k (Undef (UndefExpr E e1)) m)). {
-      eapply rtc_l; [|apply rtc_refl].
-      subst.
-      apply cstep_expr_undef; assumption.
-    }
-    * inversion H7.
-    * destruct H7 as [S'' H7].
-      inversion H7.
+  + elim H13; clear H13.
+    eapply expr_equiv_subexpr_imm_safe with (1:=H12) (2:=H); try (eassumption || reflexivity).
+    apply ch2o_safe_state_subexpr_safe with (1:=H0).
 Qed.
 
-Lemma eval_soundness' Q n e ė k ḳ m ṁ f:
-  expr_equiv e ė →
+Lemma eval_soundness_cast_int Q n e ė k ḳ m ṁ ẽ f:
+  expr_equiv e ė Int →
+  mem_equiv (mem_unlock_all m) ṁ →
+  env_equiv ẽ ê (locals k) →
+  ∀(Hlocals_alive: Forall (λ iτ, index_alive '{m} (iτ.1)) (locals k)),
   ch2o_safe_state Γ δ Q (State k (Expr (cast{sintT%T} e)) m) →
-  (∀ z n',
+  (∀ n',
    n' ≤ n →
+   ∀ Ω z m' ṁ',
    int_typed z (sintT: int_type K) →
-   ch2o_safe_state Γ δ Q (State k (Expr (# intV{sintT} z)) m) →
-   compcertc_safe_state_n Q p n' (ExprState f (Eval (Vint (Int.repr z)) (Tint I32 Signed noattr)) ḳ empty_env ṁ)) →
-  compcertc_safe_state_n Q p n (ExprState f ė ḳ empty_env ṁ).
+   ∀(Hlocals_alive: Forall (λ iτ, index_alive '{m'} (iτ.1)) (locals k)),
+   ch2o_safe_state Γ δ Q (State k (Expr (#{ Ω } (intV{sintT} z))) m') →
+   mem_equiv (mem_unlock_all m') ṁ' →
+   compcertc_safe_state_n Q p n' (ExprState f (Eval (Vint (Int.repr z)) tint) ḳ ẽ ṁ')) →
+  compcertc_safe_state_n Q p n (ExprState f ė ḳ ẽ ṁ).
 Proof.
-revert e ė.
+revert e ė m ṁ.
 apply well_founded_induction with (1:=lt_wf) (a:=n).
 clear n.
 intros n IH.
-intros.
+intros e ė m ṁ ? Hmem_equiv Henv_equiv; intros.
+case_eq (match ė with Eval _ _ => true | _ => false end); intros HEval. {
+  inversion H; clear H; subst; try discriminate.
+  * eapply H1 with (n':=n); try eauto.
+    intro; intros.
+    apply H0.
+    eapply rtc_l; try eassumption.
+    apply cstep_expr_head with (E:=[]).
+    constructor.
+    assumption.
+  * eapply ch2o_safe_state_subexpr_safe with (E:=[]) in H0. 2:{
+      reflexivity.
+    } 2:{ constructor. constructor. }
+    inversion H0; clear H0; subst.
+    inversion H; clear H; subst.
+    inversion H7.
+    discriminate.
+}
 intros t s HstarN.
 inversion HstarN; subst.
 - (* refl *)
-  destruct (compcertc_expr_never_stuck f ė ḳ empty_env ṁ).
-  + destruct H2 as [v [ty H2]].
+  destruct (compcertc_expr_never_stuck f ė ḳ ẽ ṁ).
+  + destruct H2 as [v [ty H3]].
     subst.
-    inversion H; clear H; subst.
-    unfold compcertc_safe_state_n in H1.
-    eapply H1 with (n':=0) (trace:=[]); try eauto.
-    intro; intros; eapply H0.
-    eapply rtc_l; try eassumption.
-    apply cstep_expr_head with (E:=[]).
-    constructor.
-    apply H4.
+    discriminate.
   + tauto.
-- case_eq (match ė with Eval _ _ => true | _ => false end); intros. {
-    inversion H; clear H; subst; try discriminate.
-    unfold compcertc_safe_state_n in H1.
-    eapply H1 with (n':=S n0) (4:=HstarN); try eauto.
-    intro; intros; eapply H0.
-    eapply rtc_l; try eassumption.
-    apply cstep_expr_head with (E:=[]).
-    constructor.
-    apply H5.
-  }
-  destruct H2. 2:{
+- destruct H2. 2:{
     inversion H2; subst; discriminate.
   }
   inversion H2; clear H2; subst.
-  + (* step_lred *)
-    eapply expr_equiv_no_LV_context in H; [elim H; reflexivity | assumption].
-  + (* step_rred *)
-    edestruct (rred_safe _ _ H) as [E [e1 [e2 [He1 [He1e2 [Hee' Hṁ']]]]]]; try (eassumption || reflexivity).
+  + (* step_Lred *)
+    rename m' into ṁ'.
+    edestruct (lrred_safe _ _ _ H) as [E [e1 [e2 [m' [He1 [He1e2 [Hee' [Hṁ' Hlocals_alive']]]]]]]]; try (eassumption || reflexivity). {
+      apply lrred_lred.
+      eassumption.
+    } {
+      intros.
+      eapply ch2o_safe_state_subexpr_safe with (1:=H0) (3:=H4) (E:=E ++ [CCast (sintT%T)]).
+      rewrite H2.
+      rewrite subst_snoc; reflexivity.
+    }
     unfold compcertc_safe_state_n in IH.
     subst.
-    eapply IH with (2:=Hee') (5:=H3).
+    eapply IH with (2:=Hee') (8:=H3); try eassumption.
     * lia.
+    * rewrite Hlocals_alive'; assumption.
     * intro S'.
       intro HS'.
       apply H0.
@@ -758,47 +1783,187 @@ inversion HstarN; subst.
       rewrite 2 H2.
       apply cstep_expr_head.
       apply He1e2.
-    * intros z n' Hn'.
-      apply (H1 z n'); lia.
-  + (* step_call *)
-    apply expr_equiv_no_call with (2:=H12) (3:=H13) in H.
-    elim H; reflexivity.
-  + elim H13.
-    eapply expr_equiv_imm_safe with (1:=H) (2:=H12). { reflexivity. }
-    intros.
-    destruct (classic (Γ \ locals k ⊢ₕ safe e1, m)); try eassumption.
-    destruct (H0 (State k (Undef (UndefExpr (E ++ [CCast sintT]) e1)) m)). {
-      eapply rtc_l; [|apply rtc_refl].
-      subst.
-      assert (cast{sintT%T} (subst E e1) = subst (E ++ [CCast sintT]) e1)%E. rewrite subst_snoc; reflexivity.
-      rewrite H2.
-      apply cstep_expr_undef; assumption.
+    * intros n' Hn'.
+      apply (H1 n'); lia.
+  + (* step_rred *)
+    rename m' into ṁ'.
+    edestruct (lrred_safe _ _ _ H) as [E [e1 [e2 [m' [He1 [He1e2 [Hee' [Hṁ' Hlocals_alive']]]]]]]]; try (eassumption || reflexivity). {
+      apply lrred_rred; eassumption.
+    } { 
+      intros; subst.
+      apply ch2o_safe_state_subexpr_safe with (1:=H0) (E:=E++[CCast (sintT%T)]) (3:=H4).
+      rewrite subst_snoc; reflexivity.
     }
-    * inversion H7.
-    * destruct H7 as [S'' H7].
-      inversion H7.
+    unfold compcertc_safe_state_n in IH.
+    subst.
+    eapply IH with (2:=Hee') (8:=H3); try eassumption.
+    * lia.
+    * rewrite Hlocals_alive'; assumption.
+    * intro S'.
+      intro HS'.
+      apply H0.
+      eapply rtc_l; try eassumption.
+      assert (∀ e, cast{sintT%T} (subst E e) = subst (E ++ [CCast (sintT%T)]) e)%E. {
+        intros; rewrite subst_snoc.
+        reflexivity.
+      }
+      rewrite 2 H2.
+      apply cstep_expr_head.
+      apply He1e2.
+    * intros n' Hn'.
+      apply (H1 n'); lia.
+  + (* step_call *)
+    apply expr_equiv_no_call with (2:=H11) (3:=H12) in H.
+    elim H; reflexivity.
+  + elim H12; clear H12.
+    eapply expr_equiv_subexpr_imm_safe with (1:=H11) (2:=H); try (eassumption || reflexivity).
+    intros; subst.
+    apply ch2o_safe_state_subexpr_safe with (1:=H0) (3:=H4) (E:=E++[CCast (sintT%T)]).
+    rewrite subst_snoc; reflexivity.
+Qed.
+
+Lemma eval_soundness_cast_void Q n e ė k ḳ m ṁ ẽ f:
+  expr_equiv e ė Int →
+  mem_equiv (mem_unlock_all m) ṁ →
+  env_equiv ẽ ê (locals k) →
+  ∀(Hlocals_alive: Forall (λ iτ, index_alive '{m} (iτ.1)) (locals k)),
+  ch2o_safe_state Γ δ Q (State k (Expr (cast{voidT%T} e)) m) →
+  (∀ n',
+   n' ≤ n →
+   ∀ Ω v ṿ ty m' ṁ',
+   ∀(Hlocals_alive: Forall (λ iτ, index_alive '{m'} (iτ.1)) (locals k)),
+   ch2o_safe_state Γ δ Q (State k (Expr (#{ Ω } v)) m') →
+   mem_equiv (mem_unlock_all m') ṁ' →
+   compcertc_safe_state_n Q p n' (ExprState f (Eval ṿ ty) ḳ ẽ ṁ')) →
+  compcertc_safe_state_n Q p n (ExprState f ė ḳ ẽ ṁ).
+Proof.
+revert e ė m ṁ.
+apply well_founded_induction with (1:=lt_wf) (a:=n).
+clear n.
+intros n IH.
+intros e ė m ṁ ? Hmem_equiv Henv_equiv; intros.
+case_eq (match ė with Eval _ _ => true | _ => false end); intros HEval. {
+  inversion H; clear H; subst; try discriminate.
+  * eapply H1 with (n':=n); try eauto.
+    intro; intros.
+    apply H0.
+    eapply rtc_l; try eassumption.
+    apply cstep_expr_head with (E:=[]).
+    constructor.
+    constructor.
+  * eapply ch2o_safe_state_subexpr_safe with (E:=[]) in H0. 2:{
+      reflexivity.
+    } 2:{ constructor. constructor. }
+    inversion H0; clear H0; subst.
+    inversion H; clear H; subst.
+    inversion H7.
+}
+intros t s HstarN.
+inversion HstarN; subst.
+- (* refl *)
+  destruct (compcertc_expr_never_stuck f ė ḳ ẽ ṁ).
+  + destruct H2 as [v [ty H3]].
+    subst.
+    discriminate.
+  + tauto.
+- destruct H2. 2:{
+    inversion H2; subst; discriminate.
+  }
+  inversion H2; clear H2; subst.
+  + (* step_Lred *)
+    rename m' into ṁ'.
+    edestruct (lrred_safe _ _ _ H) as [E [e1 [e2 [m' [He1 [He1e2 [Hee' [Hṁ' Hlocals_alive']]]]]]]]; try (eassumption || reflexivity). {
+      apply lrred_lred.
+      eassumption.
+    } {
+      intros.
+      eapply ch2o_safe_state_subexpr_safe with (1:=H0) (3:=H4) (E:=E ++ [CCast (voidT%T)]).
+      rewrite H2.
+      rewrite subst_snoc; reflexivity.
+    }
+    unfold compcertc_safe_state_n in IH.
+    subst.
+    eapply IH with (2:=Hee') (8:=H3); try eassumption.
+    * lia.
+    * rewrite Hlocals_alive'; assumption.
+    * intro S'.
+      intro HS'.
+      apply H0.
+      eapply rtc_l; try eassumption.
+      assert (∀ e, cast{voidT%T} (subst E e) = subst (E ++ [CCast (voidT%T)]) e)%E. {
+        intros; rewrite subst_snoc.
+        reflexivity.
+      }
+      rewrite 2 H2.
+      apply cstep_expr_head.
+      apply He1e2.
+    * intros n' Hn'.
+      apply (H1 n'); lia.
+  + (* step_rred *)
+    rename m' into ṁ'.
+    edestruct (lrred_safe _ _ _ H) as [E [e1 [e2 [m' [He1 [He1e2 [Hee' [Hṁ' Hlocals_alive']]]]]]]]; try (eassumption || reflexivity). {
+      apply lrred_rred; eassumption.
+    } { 
+      intros; subst.
+      apply ch2o_safe_state_subexpr_safe with (1:=H0) (E:=E++[CCast (voidT%T)]) (3:=H4).
+      rewrite subst_snoc; reflexivity.
+    }
+    unfold compcertc_safe_state_n in IH.
+    subst.
+    eapply IH with (2:=Hee') (8:=H3); try eassumption.
+    * lia.
+    * rewrite Hlocals_alive'; assumption.
+    * intro S'.
+      intro HS'.
+      apply H0.
+      eapply rtc_l; try eassumption.
+      assert (∀ e, cast{voidT%T} (subst E e) = subst (E ++ [CCast (voidT%T)]) e)%E. {
+        intros; rewrite subst_snoc.
+        reflexivity.
+      }
+      rewrite 2 H2.
+      apply cstep_expr_head.
+      apply He1e2.
+    * intros n' Hn'.
+      apply (H1 n'); lia.
+  + (* step_call *)
+    apply expr_equiv_no_call with (2:=H11) (3:=H12) in H.
+    elim H; reflexivity.
+  + elim H12; clear H12.
+    eapply expr_equiv_subexpr_imm_safe with (1:=H11) (2:=H); try (eassumption || reflexivity).
+    intros; subst.
+    apply ch2o_safe_state_subexpr_safe with (1:=H0) (3:=H4) (E:=E++[CCast (voidT%T)]).
+    rewrite subst_snoc; reflexivity.
 Qed.
 
 Lemma stmt_soundness Q f s ṡ:
   stmt_equiv s ṡ →
-  ∀ n k ḳ m ṁ,
+  ∀ n k ḳ m ṁ ẽ,
+  mem_equiv (mem_unlock_all m) ṁ →
+  env_equiv ẽ ê (locals k) →
+  ∀(Hlocals_alive: Forall (λ iτ, index_alive '{m} (iτ.1)) (locals k)),
   ch2o_safe_state Γ δ Q (State k (Stmt ↘ s) m) →
   (∀ n',
    n' ≤ n →
-   ch2o_safe_state Γ δ Q (State k (Stmt ↗ s) m) →
-   compcertc_safe_state_n Q p n' (Csem.State f Sskip ḳ empty_env ṁ)) →
-  (∀ n' z ḳ',
+   ∀ m' ṁ',
+   ∀(Hlocals_alive: Forall (λ iτ, index_alive '{m'} (iτ.1)) (locals k)),
+   ch2o_safe_state Γ δ Q (State k (Stmt ↗ s) m') →
+   mem_equiv (mem_unlock_all m') ṁ' →
+   compcertc_safe_state_n Q p n' (Csem.State f Sskip ḳ ẽ ṁ')) →
+  (∀ n',
    n' ≤ n →
+   ∀ z ḳ' m' ṁ',
    int_typed z (sintT: int_type K) →
    call_cont ḳ' = call_cont ḳ →
-   ch2o_safe_state Γ δ Q (State k (Stmt (⇈ (intV{sintT} z)) s) m) →
-   compcertc_safe_state_n Q p n' (ExprState f (Eval (Vint (Int.repr z)) tint) (Kreturn ḳ') empty_env ṁ)) →
-  compcertc_safe_state_n Q p n (Csem.State f ṡ ḳ empty_env ṁ).
+   mem_equiv (mem_unlock_all m') ṁ' →
+   ∀(Hlocals_alive: Forall (λ iτ, index_alive '{m'} (iτ.1)) (locals k)),
+   ch2o_safe_state Γ δ Q (State k (Stmt (⇈ (intV{sintT} z)) s) m') →
+   compcertc_safe_state_n Q p n' (ExprState f (Eval (Vint (Int.repr z)) tint) (Kreturn ḳ') ẽ ṁ')) →
+  compcertc_safe_state_n Q p n (Csem.State f ṡ ḳ ẽ ṁ).
 Proof.
 (* TODO: When adding support for loops, we'll need to perform well-founded induction on n here as well. *)
-induction 1.
+induction 1; intros n k ḳ m ṁ ẽ Hmem_equiv Henv_equiv; intros.
 - (* return *)
-  intros.
   intro; intros.
   inversion H3; clear H3; subst. {
     right.
@@ -807,24 +1972,27 @@ induction 1.
     constructor.
   }
   inversion H4; clear H4; subst; inversion H3; clear H3; subst; try intuition discriminate.
-  eapply eval_soundness'; try eassumption. {
+  eapply eval_soundness_cast_int with (k:=CExpr (cast{sintT%T} e) CReturnE :: k); try eassumption. {
     intro; intros.
     eapply H0.
     eapply rtc_l; [|eassumption].
     apply cstep_expr with (E:=CReturnE).
   }
   intros.
-  eapply H2; try eassumption.
+  eapply H2 with (m':=mem_unlock Ω m'); try eassumption.
   + lia.
   + reflexivity.
+  + rewrite mem_unlock_all_mem_unlock.
+    eassumption.
+  + rewrite mem_unlock_memenv_of.
+    assumption.
   + intro; intros.
     eapply H6.
     eapply rtc_l; [|eassumption].
-    rewrite <- mem_unlock_empty at 2.
     constructor.
 - (* skip *)
   intros.
-  eapply H0.
+  eapply H0; try eassumption.
   + reflexivity.
   + intro; intros.
     eapply H.
@@ -840,44 +2008,44 @@ induction 1.
     constructor.
   }
   inversion H5; clear H5; subst; inversion H4; clear H4; subst; try intuition discriminate.
-  eapply IHstmt_equiv1; try eassumption. {
+  eapply IHstmt_equiv1 with (n:=n0) (ḳ:=Kseq ṡ2 ḳ). 4:{
     intro; intros.
     eapply H1.
     eapply rtc_l; [|eassumption].
     constructor.
-  } 2:{
+  } { eassumption. } { eassumption. } { eassumption. } 2:{
     intros.
-    simpl in H7.
-    eapply H3; try eassumption.
-    - lia.
-    - intro; intros.
-      eapply H8.
-      eapply rtc_l; [|eassumption].
-      constructor.
+    eapply H3; try eassumption. { lia. }
+    intro; intros.
+    eapply H9.
+    eapply rtc_l; [|eassumption].
+    constructor.
+  } 2:{
+    eassumption.
   }
   intros.
   intro; intros.
-  inversion H7; clear H7; subst. {
+  inversion H8; clear H8; subst. {
     right.
     eexists; eexists.
     right.
     constructor.
   }
-  inversion H8; clear H8; subst; inversion H7; clear H7; subst. 2:{
-    inversion H15.
+  inversion H9; clear H9; subst; inversion H8; clear H8; subst. 2:{
+    inversion H16.
   }
-  eapply IHstmt_equiv2; try eassumption. {
+  eapply IHstmt_equiv2. 4:{
     intro; intros.
     eapply H5.
     eapply rtc_l; [|eassumption].
     constructor.
-  } 2:{
+  } { eassumption. } { eassumption. } { eassumption. } 3:{ eassumption. } 2:{
     intros.
     intro; intros.
     eapply H3; try eassumption.
     + lia.
     + intro; intros.
-      eapply H11.
+      eapply H13.
       eapply rtc_l; [|eassumption].
       constructor.
   }
@@ -885,7 +2053,7 @@ induction 1.
   eapply H2; try eassumption.
   + lia.
   + intro; intros.
-    eapply H8.
+    eapply H9.
     eapply rtc_l; [|eassumption].
     constructor.
 - (* if *)
@@ -898,7 +2066,7 @@ induction 1.
     constructor.
   }
   inversion H6; clear H6; subst; inversion H5; clear H5; subst; try intuition discriminate.
-  eapply eval_soundness; try eassumption. {
+  eapply eval_soundness with (k:=CExpr e (CIfE s1 s2) :: k); try eassumption. {
     intro; intros.
     eapply H2.
     eapply rtc_l; [|eassumption].
@@ -906,96 +2074,922 @@ induction 1.
   }
   intros.
   intro; intros.
-  inversion H9; clear H9; subst. {
+  inversion H10; clear H10; subst. {
     right.
-    eexists; eexists.
-    right.
-    constructor.
-    unfold bool_val.
-    simpl.
-    reflexivity.
+    inversion H8; clear H8; subst.
+    - eexists; eexists.
+      right.
+      eapply step_ifthenelse_2.
+      unfold bool_val.
+      simpl.
+      reflexivity.
+    - edestruct H6.
+      + eapply rtc_l.
+        * apply cstep_expr_if_indet.
+          intro.
+          inversion H8.
+        * apply rtc_refl.
+      + inversion H8.
+      + destruct H8.
+        inversion H8.
   }
-  inversion H10; clear H10; subst; inversion H9; clear H9; subst. {
-    inversion H19; clear H19; subst; try discriminate.
+  inversion H11; clear H11; subst; inversion H10; clear H10; subst. {
+    inversion H8; subst; inversion H20; clear H20; subst; try discriminate.
   } {
-    inversion H19; clear H19; subst; try discriminate.
-    subst.
-    inversion H18; clear H18; subst.
+    inversion H8; subst; inversion H20; clear H20; subst; try discriminate;
+    subst;
+    inversion H19; clear H19; subst.
   } {
-    inversion H19; clear H19; subst; try discriminate.
-    subst.
-    inversion H18; clear H18; subst.
+    inversion H8; subst; inversion H20; clear H20; subst; try discriminate;
+    subst;
+    inversion H19; clear H19; subst.
   } {
-    inversion H18; clear H18; subst; try discriminate.
-    subst.
-    elim H19; constructor.
+    inversion H8; subst; inversion H19; clear H19; subst; try discriminate;
+    subst;
+    elim H20; constructor.
   }
+  inversion H8; subst; try discriminate.
   unfold bool_val in H21.
   simpl in H21.
   injection H21; clear H21; intros; subst.
-  rewrite Int.eq_signed in H11.
-  rewrite Int.signed_repr in H11. 2:{
+  rewrite Int.eq_signed in H12.
+  rewrite Int.signed_repr in H12. 2:{
     apply int_typed_limits; assumption.
   }
-  rewrite Int.signed_zero in H11.
-  destruct (Coqlib.zeq z 0); simpl in H11.
+  rewrite Int.signed_zero in H12.
+  destruct (Coqlib.zeq z 0); simpl in H12.
   + (* z = 0 *)
     subst.
-    eapply IHstmt_equiv2; try eassumption. {
+    eapply IHstmt_equiv2. 7:{ eassumption. } 4:{
       intro; intros.
-      eapply H8.
+      eapply H6.
       eapply rtc_l; [|eassumption].
-      constructor.
+      apply cstep_expr_if_false.
       - simpl. constructor.
       - constructor.
+    } {
+      rewrite mem_unlock_all_mem_unlock; eassumption.
+    } {
+      eassumption.
+    } {
+      rewrite mem_unlock_memenv_of.
+      assumption.
     } 2:{
       intros.
       eapply H4; try eassumption.
       - lia.
       - intro; intros.
-        eapply H13.
+        eapply H16.
         eapply rtc_l; [|eassumption].
-        rewrite mem_unlock_empty.
         constructor.
     }
     intros.
-    rewrite mem_unlock_empty in H10.
-    intro; intros.
     eapply H3; try eassumption.
     * lia.
     * intro; intros.
-      eapply H10.
+      eapply H13.
       eapply rtc_l; [|eassumption].
       constructor.
   + (* z ≠ 0 *)
-    eapply IHstmt_equiv1; try eassumption. {
+    eapply IHstmt_equiv1. 7:{ eassumption. } 4:{
       intro; intros.
-      eapply H8.
+      eapply H6.
       eapply rtc_l; [|eassumption].
       constructor.
       - constructor.
       - intro.
         elim n1.
-        inversion H10; clear H10; subst.
+        inversion H13; clear H13; subst.
         reflexivity.
+    } {
+      rewrite mem_unlock_all_mem_unlock.
+      eassumption.
+    } {
+      eassumption.
+    } {
+      rewrite mem_unlock_memenv_of; assumption.
     } 2:{
       intros.
       eapply H4; try eassumption.
       - lia.
       - intro; intros.
-        eapply H13.
+        eapply H16.
         eapply rtc_l; [|eassumption].
-        rewrite mem_unlock_empty.
         constructor.
     }
     intros.
-    rewrite mem_unlock_empty in H10.
     eapply H3; try eassumption.
     * lia.
     * intro; intros.
-      eapply H10.
+      eapply H13.
       eapply rtc_l; [|eassumption].
       constructor.
+- intro; intros.
+  inversion H3; clear H3; subst. {
+    right.
+    eexists; eexists; right.
+    constructor.
+  }
+  inversion H4; clear H4; subst; inversion H3; clear H3; subst; try destruct H12; try discriminate.
+  eapply eval_soundness_cast_void with (k:=CExpr (cast{voidT%T} e) CDoE :: k). eassumption. eassumption. 5:{ eassumption. } 3:{
+    intro; intros.
+    eapply H0.
+    eapply rtc_l.
+    - eapply cstep_expr with (E:=CDoE).
+    - eassumption.
+  } { eassumption. } { eassumption. }
+  intros.
+  intro; intros.
+  inversion H7; clear H7; subst. {
+    right.
+    eexists; eexists; right.
+    constructor.
+  }
+  inversion H8; clear H8; subst; inversion H7; clear H7; subst; try discriminate. {
+    inversion H17; clear H17; subst; try discriminate.
+  } {
+    inversion H17; clear H17; subst; try discriminate; subst.
+    inversion H16; clear H16; subst.
+  } {
+    inversion H17; clear H17; subst; try discriminate.
+    subst.
+    inversion H16.
+  } {
+    inversion H16; clear H16; subst; try discriminate.
+    subst.
+    elim H17.
+    constructor.
+  }
+  eapply H1. 5:{
+    eassumption.
+  } { lia. } 2:{
+    intro; intros.
+    eapply H4; try eassumption.
+    eapply rtc_l.
+    * constructor.
+    * eassumption.
+  } {
+    rewrite mem_unlock_memenv_of; assumption.
+  }
+  rewrite mem_unlock_all_mem_unlock.
+  eassumption.
+Qed.
+
+End Locals.
+
+Lemma mem_lookup_mem_alloc_ne m b v b1:
+  b1 ≠ b →
+  m !!{Γ} addr_top (N.pos b) sintT = Some v →
+  mem_alloc Γ (N.pos b1) false perm_full (val_new Γ sintT) m
+    !!{Γ} addr_top (N.pos b) sintT = Some v.
+Proof.
+  intros ?.
+  destruct m as [m].
+  simpl.
+  unfold mem_lookup.
+  simpl.
+  unfold cmap_lookup.
+  rewrite option_guard_True. 2:{ constructor. simpl. lia. }
+  simpl.
+  rewrite lookup_insert_ne. 2:{ congruence. }
+  tauto.
+Qed.
+
+Lemma mem_lookup_mem_free o m o' v:
+  o' ≠ o →
+  m !!{Γ} addr_top o sintT = Some v →
+  mem_free o' m !!{Γ} addr_top o sintT = Some v.
+Proof.
+  intros ?.
+  destruct m as [m].
+  simpl.
+  unfold mem_lookup.
+  simpl.
+  unfold cmap_lookup.
+  rewrite option_guard_True. 2:{ constructor. simpl. lia. }
+  simpl.
+  rewrite lookup_alter_ne with (1:=H).
+  destruct (m !! o) as [[|w μ]|]; try (intros; tauto).
+Qed.
+
+Lemma mem_writable_mem_free o o' m:
+  o' ≠ o →
+  mem_writable Γ (addr_top o sintT) m →
+  mem_writable Γ (addr_top o sintT) (mem_free o' m).
+Proof.
+  destruct m as [m].
+  unfold mem_writable.
+  intros.
+  destruct H0 as [w [? ?]].
+  exists w.
+  split.
+  - unfold mem_free.
+    simpl.
+    unfold cmap_lookup.
+    rewrite option_guard_True. 2:{ constructor. simpl. lia. }
+    simpl.
+    rewrite lookup_alter_ne with (1:=H).
+    simpl in H0.
+    unfold cmap_lookup in H0.
+    rewrite option_guard_True in H0. 2:{ constructor. simpl. lia. }
+    simpl in H0.
+    assumption.
+  - assumption.
+Qed.
+
+Lemma list_norepet_rev {A} (xs: list A):
+  Coqlib.list_norepet xs → Coqlib.list_norepet (rev xs).
+Proof.
+  induction xs; simpl; intros.
+  - constructor.
+  - inversion H; clear H; subst.
+    apply Coqlib.list_norepet_append_commut.
+    constructor.
+    + intro.
+      elim H2.
+      apply In_rev.
+      assumption.
+    + auto.
+Qed.
+
+Lemma free_list_app_elim ṁ0 xs ys ṁ2:
+  Memory.Mem.free_list ṁ0 (xs ++ ys) = Some ṁ2 →
+  ∃ ṁ1,
+  Memory.Mem.free_list ṁ0 xs = Some ṁ1 /\
+  Memory.Mem.free_list ṁ1 ys = Some ṁ2.
+Proof.
+  revert ṁ0.
+  induction xs; intros.
+  - exists ṁ0.
+    split. {
+      reflexivity.
+    }
+    assumption.
+  - inversion H; clear H; subst.
+    destruct a.
+    destruct p0.
+    case_eq (Memory.Mem.free ṁ0 b z0 z); intros; rewrite H in H1; try discriminate.
+    rename m into ṁ0'.
+    destruct (IHxs _ H1) as [ṁ1 [? ?]].
+    exists ṁ1.
+    split. {
+      simpl.
+      rewrite H.
+      assumption.
+    }
+    congruence.
+Qed.
+
+Lemma free_list_app_intro ṁ0 xs ṁ1 ys ṁ2:
+  Memory.Mem.free_list ṁ0 xs = Some ṁ1 →
+  Memory.Mem.free_list ṁ1 ys = Some ṁ2 →
+  Memory.Mem.free_list ṁ0 (xs ++ ys) = Some ṁ2.
+Proof.
+  revert ṁ0.
+  induction xs; intros.
+  - simpl in H.
+    inversion H; clear H; subst.
+    assumption.
+  - inversion H; clear H; subst.
+    destruct a.
+    destruct p0.
+    case_eq (Memory.Mem.free ṁ0 b z0 z); intros; rewrite H in H2; try discriminate.
+    rename m into ṁ0'.
+    simpl.
+    rewrite H.
+    apply IHxs; assumption.
+Qed.
+
+Lemma index_alive_dom o (m: mem K):
+  index_alive '{m} o → o ∈ dom indexset m.
+Proof.
+  intros.
+  destruct (classic (o ∈ dom indexset m)); try assumption.
+  apply mem_allocable_memenv_of in H0.
+  unfold index_alive in H.
+  destruct H as [τ H].
+  congruence.
+Qed.
+
+Lemma list_norepet_map {A B} (f: A -> B) xs:
+  Coqlib.list_norepet (map f xs) →
+  Coqlib.list_norepet xs.
+Proof.
+  induction xs; intros.
+  - constructor.
+  - inversion H; clear H; subst.
+    apply IHxs in H3.
+    constructor.
+    + intro.
+      elim H2.
+      apply in_map.
+      assumption.
+    + assumption.
+Qed.
+
+Lemma elem_of_list_In {A} x (xs: list A):
+  elem_of_list x xs ↔ In x xs.
+Proof.
+  induction xs; intros; split; intros.
+  - inversion H.
+  - inversion H.
+  - inversion H; clear H; subst.
+    + left; reflexivity.
+    + right; tauto.
+  - inversion H; clear H; subst.
+    + left; reflexivity.
+    + right; tauto.
+Qed.
+
+Lemma alloc_variables_soundness Q f ê ê' s ṡ:
+  Coqlib.list_norepet (ê ++ ê') →
+  stmt_equiv (rev (ê ++ ê')) s ṡ →
+  ∀ n k ḳ m ṁ0 ṁ ẽ0 ẽ,
+  mem_equiv (mem_unlock_all m) ṁ0 →
+  ∀(Hblocks_norepet: ∀ i x, rev ê !! i = Some x → ∃ b, Maps.PTree.get x ẽ0 = Some (b, tint) /\ (Memory.Mem.nextblock ṁ0 = b + Pos.of_succ_nat i)%positive),
+  ∀(Henv_tight: ∀ x b τ, Maps.PTree.get x ẽ0 = Some (b, τ) → x ∈ ê),
+  env_equiv ẽ0 (rev ê) (locals k) →
+  alloc_variables (globalenv p) ẽ0 ṁ0 (map (λ x, (x, tint)) ê') ẽ ṁ →
+  ∀(Hlocals_alive: Forall (λ iτ, index_alive '{m} (iτ.1)) (locals k)),
+  ch2o_safe_state Γ δ Q (State k (Stmt ↘ (Nat.iter (length ê') (λ s, local{sintT} s) s)) m) →
+  (∀ m',
+   ch2o_safe_state Γ δ Q (State k (Stmt ↗ (Nat.iter (length ê') (λ s, local{sintT} s) s)) m') →
+   False) →
+  (∀ n',
+   n' ≤ n →
+   ∀ z ḳ' m' ṁ',
+   int_typed z (sintT: int_type K) →
+   call_cont ḳ' = call_cont ḳ →
+   ∀(Hblocks_norepet: ∀ i x, rev (ê ++ ê') !! i = Some x → ∃ b, Maps.PTree.get x ẽ = Some (b, tint) /\ (Memory.Mem.nextblock ṁ = b + Pos.of_succ_nat i)%positive),
+   ∀(Henv_tight: ∀ x b τ, Maps.PTree.get x ẽ = Some (b, τ) → x ∈ (ê ++ ê')%list),
+   (∀ x, In x ê → Maps.PTree.get x ẽ = Maps.PTree.get x ẽ0) →
+   (∀ x,
+    In x ê' →
+    match Maps.PTree.get x ẽ with
+      None => True
+    | Some (b, τ) => ¬ index_alive '{m'} (N.pos b) /\ Memory.Mem.range_perm ṁ' b 0 (sizeof (globalenv p) τ) Memtype.Cur Memtype.Freeable
+    end) →
+   mem_equiv (mem_unlock_all m') ṁ' →
+   ∀(Hlocals_alive: Forall (λ iτ, index_alive '{m'} (iτ.1)) (locals k)),
+   ch2o_safe_state Γ δ Q (State k (Stmt (⇈ (intV{sintT} z)) (Nat.iter (length ê') (λ s, local{sintT} s) s)) m') →
+   compcertc_safe_state_n Q p n' (ExprState f (Eval (Vint (Int.repr z)) tint) (Kreturn ḳ') ẽ ṁ')) →
+  compcertc_safe_state_n Q p n
+    (Csem.State f (Ssequence ṡ (Sreturn (Some (Eval (Vint (Int.repr 0)) tint)))) ḳ ẽ ṁ).
+Proof.
+  revert ê' ê.
+  induction ê'; intros.
+  - intro; intros.
+    inversion H7; clear H7; subst. {
+      right.
+      eexists; eexists.
+      right.
+      constructor.
+    }
+    inversion H8; clear H8; subst; inversion H7; clear H7; subst; try (destruct H16); try discriminate.
+    inversion H3; clear H3; subst.
+    eapply stmt_soundness. 8:{ eassumption. } eassumption. eassumption. {
+      rewrite app_nil_r. eassumption.
+    } eassumption. eassumption. 2:{
+      intros.
+      eapply H6. lia. assumption. assumption. {
+        rewrite app_nil_r. apply Hblocks_norepet.
+      } {
+        rewrite app_nil_r. apply Henv_tight.
+      } reflexivity. { intros. inversion H12. } eassumption.
+      assumption. assumption.
+    }
+    intros.
+    (* Ssequence *)
+    apply H5 in H7.
+    tauto.
+  - rename a into x.
+    simpl in H3.
+    inversion H3; clear H3; subst.
+    rename m1 into ṁ0'.
+    destruct H1.
+    assert (Hdom: (N.pos b1: index) ∉ dom indexset m). {
+      rewrite <- dom_mem_unlock_all.
+      apply domains_equiv0.
+      rewrite Memory.Mem.alloc_result with (1:=H14).
+      reflexivity.
+    }
+    eapply IHê' with (ê:=(ê ++ [x])%list). {
+     rewrite <- app_assoc. assumption.
+    } {
+      rewrite <- app_assoc. assumption.
+    } 5:{
+      eassumption.
+    } 6:{
+      intro; intros.
+      eapply H4.
+      eapply rtc_l; [|eassumption].
+      apply cstep_in_block with (o:=Npos b1).
+      - constructor.
+      - assumption.
+    } {
+      split.
+      - intros.
+        destruct (classic (b = b1)).
+        + subst.
+          apply block_equiv_alloced with (oz:=None).
+          * apply Memory.Mem.load_alloc_same' with (1:=H14).
+            -- reflexivity.
+            -- reflexivity.
+            -- simpl.
+               apply Z.divide_0_r.
+          * intros.
+            eapply Memory.Mem.valid_access_implies.
+            apply Memory.Mem.valid_access_alloc_same with (1:=H14).
+            -- reflexivity.
+            -- reflexivity.
+            -- simpl; apply Z.divide_0_r.
+            -- constructor.
+          * intro; intros.
+            apply Memory.Mem.perm_alloc_2 with (1:=H14).
+            assumption.
+          * rewrite memenv_of_mem_unlock_all.
+            apply mem_alloc_new_index_alive'.
+            -- assumption.
+            -- constructor.
+               constructor.
+          * rewrite memenv_of_mem_unlock_all.
+            constructor.
+            -- eapply mem_alloc_new_index_typed'.
+               ++ assumption.
+               ++ constructor; constructor.
+            -- constructor; constructor.
+            -- constructor.
+            -- reflexivity.
+            -- simpl.
+               lia.
+            -- apply Nat.divide_0_r.
+            -- constructor.
+          * erewrite mem_unlock_all_lookup. reflexivity.
+            erewrite mem_lookup_alloc; try eassumption.
+            -- reflexivity.
+            -- apply val_new_typed.
+               ++ assumption.
+               ++ constructor; constructor.
+            -- constructor.
+          * apply mem_writable_unlock_all.
+            eapply mem_alloc_writable_top.
+            -- assumption.
+            -- apply val_new_typed.
+               ++ assumption.
+               ++ constructor; constructor.
+            -- constructor.
+          * constructor.
+        + destruct (blocks_equiv0 b).
+          * apply block_equiv_not_alloced.
+            rewrite memenv_of_mem_unlock_all.
+            intro.
+            elim H3.
+            erewrite mem_alloc_memenv_of in H7.
+            -- eapply mem_alloc_index_alive_inv. 2:{ rewrite memenv_of_mem_unlock_all. eassumption. }
+               congruence.
+            -- assumption.
+            -- apply val_new_typed.
+               ++ assumption.
+               ++ constructor; constructor.
+          * apply block_equiv_alloced with (oz:=oz).
+            -- apply Memory.Mem.load_alloc_other with (1:=H14) (2:=H3).
+            -- apply Memory.Mem.valid_access_alloc_other with (1:=H14).
+               assumption.
+            -- intro; intros.
+               apply Memory.Mem.perm_alloc_1 with (1:=H14).
+               apply H8; assumption.
+            -- rewrite memenv_of_mem_unlock_all.
+               erewrite mem_alloc_memenv_of.
+               ++ rewrite memenv_of_mem_unlock_all in H9.
+                  apply mem_alloc_index_alive_ne; try assumption.
+                  congruence.
+               ++ assumption.
+               ++ apply val_new_typed.
+                  ** assumption.
+                  ** constructor; constructor.
+            -- rewrite memenv_of_mem_unlock_all.
+               apply addr_top_typed.
+               ++ assumption.
+               ++ eapply memenv_forward_typed.
+                  ** apply mem_alloc_new_forward'.
+                     --- assumption.
+                     --- assumption.
+                     --- constructor; constructor.
+                  ** inversion H10; clear H10; subst.
+                     rewrite memenv_of_mem_unlock_all in H22.
+                     assumption.
+               ++ constructor; constructor.
+           -- rewrite mem_unlock_all_mem_alloc. 2:{ reflexivity. }
+              apply mem_lookup_mem_alloc_ne. { congruence. }
+              assumption.
+           -- rewrite mem_unlock_all_mem_alloc. 2:{ reflexivity. }
+              apply mem_alloc_writable.
+              ++ exact sintT%T.
+              ++ rewrite dom_mem_unlock_all.
+                 assumption.
+              ++ assumption.
+           -- assumption.
+      - intros.
+        rewrite dom_mem_unlock_all.
+        rewrite mem_dom_alloc.
+        rewrite Memory.Mem.alloc_result with (1:=H14).
+        rewrite Memory.Mem.nextblock_alloc with (1:=H14) in H1.
+        rewrite elem_of_union.
+        intro.
+        destruct H3.
+        + rewrite elem_of_singleton in H3.
+          injection H3; clear H3; intros; subst.
+          lia.
+        + rewrite <- dom_mem_unlock_all in H3.
+          apply domains_equiv0 in H3. assumption.
+          lia.
+      - rewrite mem_unlock_all_mem_alloc. 2:{ reflexivity. }
+        apply mem_alloc_new_valid'; try eassumption.
+        + rewrite dom_mem_unlock_all. assumption.
+        + apply perm_full_valid.
+        + apply perm_full_mapped.
+        + constructor; constructor.
+    } {
+      intros.
+      rewrite rev_app_distr in H1.
+      simpl in H1.
+      rewrite Memory.Mem.nextblock_alloc with (1:=H14).
+      destruct i.
+      - simpl in H1.
+        injection H1; clear H1; intros; subst.
+        rewrite Maps.PTree.gss.
+        f_equal.
+        f_equal.
+        rewrite Memory.Mem.alloc_result with (1:=H14).
+        eexists. split. reflexivity. lia.
+      - simpl in H1.
+        rewrite Maps.PTree.gso.
+        + apply Hblocks_norepet in H1.
+          unfold Values.block.
+          destruct H1 as [b0 [? ?]].
+          rewrite H1.
+          eexists; split. reflexivity.
+          lia.
+        + assert (ê ++ x :: ê' = (ê ++ [x]) ++ ê')%list. {
+            rewrite <- app_assoc.
+            reflexivity.
+          }
+          rewrite H3 in H.
+          apply Coqlib.list_norepet_append_left in H.
+          apply list_norepet_rev in H.
+          rewrite rev_app_distr in H.
+          inversion H; clear H; subst.
+          apply elem_of_list_lookup_2 in H1.
+          unfold elem_of in H1.
+          apply elem_of_list_In in H1.
+          intro; subst; tauto.
+    } {
+      intros.
+      destruct (classic (x0 = x)).
+      - subst.
+        apply elem_of_app; right.
+        constructor.
+      - rewrite Maps.PTree.gso with (1:=H3) in H1.
+        apply Henv_tight in H1.
+        apply elem_of_app; left; assumption.
+    } {
+      simpl.
+      rewrite rev_app_distr.
+      simpl.
+      constructor.
+      - apply Maps.PTree.gss.
+      - assert (ê ++ x :: ê' = (ê ++ [x]) ++ ê')%list. {
+          rewrite <- app_assoc.
+          reflexivity.
+        }
+        rewrite H1 in H.
+        apply Coqlib.list_norepet_append_left in H.
+        apply list_norepet_rev in H.
+        revert H.
+        revert H2.
+        rewrite rev_app_distr.
+        simpl.
+        generalize (locals k).
+        generalize (rev ê).
+        induction l; intros.
+        + inversion H2; clear H2; subst.
+          constructor.
+        + inversion H2; clear H2; subst.
+          inversion H; clear H; subst.
+          inversion H9; clear H9; subst.
+          constructor.
+          * rewrite Maps.PTree.gso. assumption.
+            intro; subst.
+            elim H7.
+            left.
+            reflexivity.
+          * apply IHl. assumption.
+            constructor.
+            -- intro.
+               elim H7.
+               right.
+               assumption.
+            -- assumption.
+    } {
+      constructor.
+      - eapply mem_alloc_index_alive'. assumption.
+        apply val_new_typed. assumption. { constructor; constructor. }
+      - apply Forall_impl with (1:=Hlocals_alive); intros.
+        erewrite mem_alloc_memenv_of with (τ:=sintT%T).
+        + destruct (classic (x0.1 = N.pos b1)).
+          * rewrite H3.
+            eapply mem_alloc_index_alive.
+          * eapply mem_alloc_index_alive_ne. congruence. assumption.
+        + assumption.
+        + apply val_new_typed.
+          * assumption.
+          * constructor; constructor.
+    } 2:{
+      intros.
+      destruct H10.
+      inversion Hlocals_alive0; clear Hlocals_alive0; subst.
+      destruct (blocks_equiv1 b1). {
+        rewrite memenv_of_mem_unlock_all in H10.
+        elim (H10 H13).
+      }
+      eapply H6. lia. assumption. assumption. {
+        rewrite <- app_assoc in Hblocks_norepet0. assumption.
+      } {
+        rewrite <- app_assoc in Henv_tight0. assumption.
+      } {
+        intros.
+        rewrite H8. 2:{ apply in_or_app. left. assumption. }
+        assert (ê ++ x :: ê' = (ê ++ [x]) ++ ê')%list. {
+          rewrite <- app_assoc.
+          reflexivity.
+        }
+        rewrite H24 in H.
+        apply Coqlib.list_norepet_append_left in H.
+        apply list_norepet_rev in H.
+        rewrite rev_app_distr in H.
+        inversion H; clear H; subst.
+        rewrite <- In_rev in H27.
+        apply Maps.PTree.gso.
+        intro; subst; tauto.
+      } 4:{
+        intro; intros.
+        eapply H11; try eassumption.
+        eapply rtc_l; [|eassumption].
+        constructor.
+        constructor.
+      } {
+        intros.
+        inversion H23; clear H23; subst.
+        - rewrite H8. 2:{ apply in_or_app. right; constructor. reflexivity. }
+          rewrite Maps.PTree.gss.
+          split.
+          + rewrite mem_free_memenv_of.
+            apply mem_free_index_alive.
+          + apply H17.
+        - apply H9 in H24.
+          destruct (Maps.PTree.get x0 ẽ) as [[b τ]|]; try trivial.
+          destruct H24.
+          split.
+          + rewrite mem_free_memenv_of.
+            intro; elim H23.
+            eapply mem_free_index_alive_inv with (1:=H25).
+          + assumption.
+      } {
+        split.
+        - intros.
+          destruct (classic (b = b1)).
+          + subst.
+            apply block_equiv_not_alloced.
+            rewrite memenv_of_mem_unlock_all.
+            rewrite mem_free_memenv_of.
+            apply mem_free_index_alive.
+          + destruct (blocks_equiv1 b).
+            * apply block_equiv_not_alloced.
+              rewrite memenv_of_mem_unlock_all.
+              rewrite memenv_of_mem_unlock_all in H24.
+              rewrite mem_free_memenv_of.
+              intro.
+              elim H24.
+              apply mem_free_index_alive_inv with (1:=H25).
+            * apply block_equiv_alloced with (oz:=oz0); try assumption.
+              -- rewrite memenv_of_mem_unlock_all.
+                 rewrite memenv_of_mem_unlock_all in H27.
+                 rewrite mem_free_memenv_of.
+                 apply mem_free_index_alive_ne. congruence.
+                 assumption.
+              -- apply addr_top_typed.
+                 ++ assumption.
+                 ++ rewrite memenv_of_mem_unlock_all.
+                    eapply memenv_forward_typed.
+                    ** rewrite mem_free_memenv_of.
+                       apply mem_free_forward.
+                    ** inversion H28; subst.
+                       rewrite memenv_of_mem_unlock_all in H38.
+                       assumption.
+                 ++ constructor; constructor.
+              -- rewrite mem_unlock_all_mem_free.
+                 apply mem_lookup_mem_free. congruence.
+                 assumption.
+              -- rewrite mem_unlock_all_mem_free.
+                 apply mem_writable_mem_free; try assumption.
+                 congruence.
+        - intros.
+          rewrite mem_unlock_all_mem_free.
+          rewrite mem_dom_free.
+          apply domains_equiv1.
+          assumption.
+        - rewrite mem_unlock_all_mem_free.
+          apply mem_free_valid'; assumption.
+      }
+      apply Forall_forall; intros.
+      rewrite Forall_forall in Hlocals_alive.
+      rewrite Forall_forall in H16.
+      rewrite mem_free_memenv_of.
+      apply mem_free_index_alive_ne.
+      - apply Hlocals_alive in H23.
+        destruct x0 as [x0 τ].
+        simpl; intro; subst.
+        rewrite Memory.Mem.alloc_result with (1:=H14) in H23.
+        simpl in H23.
+        apply index_alive_dom in H23.
+        rewrite <- dom_mem_unlock_all in H23.
+        apply domains_equiv0 in H23. tauto.
+        lia.
+      - apply H16.
+        assumption.
+    }
+    intros.
+    eapply H5.
+    intro; intros.
+    apply H1.
+    eapply rtc_l; [|eassumption].
+    constructor.
+    constructor.
+  Unshelve.
+  exact ('{m}).
+  exact ('{m}).
+  exact ('{m}).
+  exact ('{m}).
+  exact ('{m}).
+  exact ('{m}).
+Qed.
+
+Inductive program_equiv: Prop :=
+| program_equiv_intro ê s ṡ b:
+  stringmap_lookup "main" δ = Some (Nat.iter (length ê) (λ s, local{sintT} s) s) →
+  Genv.init_mem p <> None →
+  let ge := globalenv p in
+  Genv.find_symbol ge p.(prog_main) = Some b →
+  let f := {|
+    fn_return:=type_int32s;
+    fn_callconv:=AST.cc_default;
+    fn_params:=nil;
+    fn_vars:=rev (map (λ x, (x, tint)) ê);
+    fn_body:=
+      Ssequence
+        ṡ 
+        (Sreturn (Some (Eval (Vint (Int.repr 0)) (Tint I32 Signed noattr))))
+  |} in
+  Coqlib.list_norepet (var_names (fn_params f) ++ var_names (fn_vars f)) →
+  Genv.find_funct_ptr ge b = Some (Internal f) →
+  stmt_equiv ê s ṡ →
+  program_equiv.
+
+Definition globdef_is_fun{F V}(g: AST.globdef F V): bool :=
+  match g with
+    AST.Gfun _ => true
+  | AST.Gvar _ => false
+  end.
+
+Lemma init_mem_ok `{prog: Ctypes.program F}:
+  forallb (λ gd, globdef_is_fun (gd.2)) (AST.prog_defs prog) = true →
+  Genv.init_mem prog <> None.
+Proof.
+intros.
+unfold Genv.init_mem.
+assert (∀ gl ge m, (∀ g, In g gl → globdef_is_fun (snd g) = true) → Genv.alloc_globals (F:=Ctypes.fundef F) (V:=type) ge m gl <> None). {
+  induction gl; intros.
+  - simpl. intro; discriminate.
+  - simpl.
+    unfold Genv.alloc_global.
+    destruct a.
+    destruct g.
+    + case_eq (Memory.Mem.alloc m 0 1).
+      intros.
+      destruct (Memory.Mem.range_perm_drop_2 m0 b 0 1 Memtype.Nonempty).
+      * unfold Memory.Mem.range_perm.
+        intros.
+        apply Memory.Mem.perm_alloc_2 with (1:=H1) (2:=H2).
+      * rewrite e.
+        apply IHgl.
+        intros.
+        apply H0.
+        right.
+        assumption.
+    + lapply (H0 (i, AST.Gvar v)).
+      intros; discriminate. left.
+      reflexivity.
+}
+apply H0.
+rewrite -> (List.forallb_forall (A:=AST.ident * AST.globdef (Ctypes.fundef F) type)) in H.
+apply H.
+Qed.
+
+Lemma alloc_variables_not_stuck ṁ ẽ xs:
+  ∃ ẽ' ṁ', alloc_variables (globalenv p) ẽ ṁ xs ẽ' ṁ'.
+Proof.
+  revert ẽ ṁ.
+  induction xs; intros.
+  - eexists; eexists; constructor.
+  - destruct a as [x τ].
+    case_eq (Memory.Mem.alloc ṁ 0 (sizeof (globalenv p) τ)); intros ṁ' b ?.
+    destruct (IHxs (Maps.PTree.set x (b, τ) ẽ) ṁ') as [ẽ'' [ṁ'' ?]].
+    eexists; eexists; econstructor; eassumption.
+Qed.
+
+Lemma alloc_variables_app:
+  ∀ xs ẽ ṁ ys ẽ' ṁ',
+  alloc_variables (globalenv p) ẽ ṁ (xs ++ ys)%list ẽ' ṁ' →
+  ∃ ẽ'' ṁ'', alloc_variables (globalenv p) ẽ ṁ xs ẽ'' ṁ'' /\ alloc_variables (globalenv p) ẽ'' ṁ'' ys ẽ' ṁ'.
+Proof.
+  induction xs; intros.
+  - eexists; eexists.
+    split. constructor. assumption.
+  - destruct a as [x τ].
+    inversion H; clear H; subst.
+    rename m1 into ṁ'''.
+    rename b1 into b.
+    destruct (IHxs _ _ _ _ _ H8) as [ẽ'' [ṁ'' [? ?]]].
+    eexists; eexists; split.
+    + econstructor; eassumption.
+    + eassumption.
+Qed.
+
+(*
+Lemma alloc_variables_soundness :
+  alloc_variables (globalenv p) ṁ ẽ (foldr (λ x xs, ((x, tint)::xs)) [] ê) ṁ' ẽ' →
+  mem_equiv ṁ' env_equiv
+*)
+
+Lemma free_list_lemma ê ẽ ṁ (m': mem K) ṁ'0 xbτs:
+  (∀ i x, ê !! i = Some x → ∃ b, Maps.PTree.get x ẽ = Some (b, tint) /\ (Memory.Mem.nextblock ṁ = b + Pos.of_succ_nat i)%positive) →
+  (∀ x b τ, Maps.PTree.get x ẽ = Some (b, τ) → x ∈ ê) →
+  ∀(Hnorepet: Coqlib.list_norepet (map fst xbτs)),
+  (∀ xbτ,
+   In xbτ xbτs →
+   match xbτ with
+   | (x, (b, τ)) =>
+     Maps.PTree.get x ẽ = Some (b, τ) /\
+     ¬ index_alive '{m'} (N.pos b) /\ Memory.Mem.range_perm ṁ'0 b 0 (sizeof (globalenv p) τ) Memtype.Cur Memtype.Freeable
+   end) →
+  ∃ ṁ',
+  Memory.Mem.free_list ṁ'0
+  (map (block_of_binding (Smallstep.globalenv (semantics p)))
+     xbτs) = Some ṁ'.
+Proof.
+  intros ? ?.
+  revert ṁ'0.
+  induction xbτs; intros.
+  - eexists.
+    constructor.
+  - destruct a as [x [b τ]].
+    destruct (H1 (x, (b, τ))) as [? [? ?]]. { left. reflexivity. }
+    destruct Memory.Mem.range_perm_free with (1:=H4) as [ṁ'1 ?].
+    inversion Hnorepet; clear Hnorepet; subst.
+    destruct (IHxbτs ṁ'1) as [ṁ' ?]. assumption.
+    + intros.
+      destruct xbτ as [x' [b' τ']].
+      destruct (H1 (x', (b', τ'))) as [? [? ?]]. { right. assumption. }
+      split. assumption.
+      split. assumption.
+      intro; intros.
+      apply Memory.Mem.perm_free_1 with (1:=e). 2:{ apply H10; assumption. }
+      left.
+      assert (x' ≠ x). {
+        intro; subst.
+        elim H7.
+        apply in_map with (1:=H5) (f:=fst).
+      }
+      destruct (elem_of_list_lookup_1 ê x) as [i Hi]. {
+        eapply H0; eassumption.
+      }
+      destruct (elem_of_list_lookup_1 ê x') as [i' Hi']. {
+        eapply H0; eassumption.
+      }
+      assert (i' ≠ i). congruence.
+      apply H in Hi.
+      apply H in Hi'.
+      destruct Hi as [b_ [? ?]].
+      destruct Hi' as [b'_ [? ?]].
+      rewrite H14 in H2; injection H2; clear H2; intros; subst.
+      rewrite H16 in H6; injection H6; clear H6; intros; subst.
+      lia.
+    + exists ṁ'.
+      simpl.
+      destruct p. simpl in e.
+      simpl.
+      rewrite e.
+      apply H5.
 Qed.
 
 Theorem soundness Q:
@@ -1005,42 +2999,94 @@ Theorem soundness Q:
 Proof.
 intros Hequiv Hch2o.
 destruct Hequiv.
-case_eq (Genv.init_mem p); intros; try tauto. clear H0; rename H4 into H0.
+case_eq (Genv.init_mem p). 2:{ intros; tauto. }
+intros ṁ ?. clear H0; rename H4 into H0.
 econstructor. { econstructor; try eassumption. reflexivity. }
 intro n; intro; intros.
 (* Callstate *)
 inversion H4; clear H4; subst. {
   right.
+  edestruct alloc_variables_not_stuck as [? [? ?]].
   eexists.
   eexists.
   right.
   eapply step_internal_function. {
-    constructor.
+    assumption.
+  } {
+    eassumption.
   } {
     constructor.
-  } {
-    constructor.
-  }    
+  }
 }
-inversion H5; clear H5; subst; inversion H4; clear H4; subst.
-clear H1 H2 H12 H14.
-inversion H13; clear H13; subst.
-simpl in H6.
-(* Ssequence *)
-inversion H6 ; clear H6; subst. {
-  right.
-  eexists.
-  eexists.
-  right.
+inversion H6; clear H6; subst; inversion H4; clear H4; subst.
+inversion H15; clear H15; subst.
+rename m2 into ṁ1.
+rename e into ẽ.
+simpl in H7.
+(* Allocating the locals *)
+eapply alloc_variables_soundness with (ẽ0:=empty_env) (ê:=[]) (ê':=rev ê) (m:=(∅: mem K)) (ṁ0:=ṁ) (k:=[CParams "main" []]).
+12:{ eassumption. }
+- simpl.
+  simpl in H13.
+  unfold var_names in H13.
+  rewrite map_rev in H13.
+  rewrite map_map in H13.
+  simpl in H13.
+  rewrite map_id in H13.
+  assumption.
+- simpl.
+  rewrite rev_involutive.
+  eassumption.
+- split.
+  + intros.
+    apply block_equiv_not_alloced.
+    intro.
+    apply index_alive_dom in H4.
+    rewrite dom_mem_unlock_all in H4.
+    assert (dom indexset (∅: mem K) = ∅). {
+      unfold empty.
+      unfold dom.
+      unfold sep_empty.
+      unfold mem_sep_ops.
+      unfold cmap_ops.
+      simpl.
+      rewrite dom_empty_L.
+      reflexivity.
+    }
+    rewrite H6 in H4.
+    apply elem_of_empty in H4.
+    elim H4.
+  + intros.
+    rewrite dom_mem_unlock_all.
+    unfold dom.
+    unfold cmap_dom.
+    unfold empty.
+    unfold sep_empty.
+    unfold mem_sep_ops.
+    unfold cmap_ops.
+    rewrite dom_empty_L.
+    intro.
+    apply elem_of_empty in H6.
+    elim H6.
+  + rewrite mem_unlock_all_empty.
+    apply cmap_empty_valid'.
+- intros.
+  simpl in H4.
+  rewrite lookup_nil in H4.
+  discriminate.
+- intros.
+  unfold empty_env in H4.
+  rewrite Maps.PTree.gempty in H4.
+  discriminate.
+- simpl.
   constructor.
-}
-inversion H1; clear H1; subst; inversion H4; clear H4; subst.
-rename H2 into H6.
-(* Executing the body *)
-eapply stmt_soundness; try eassumption. {
-  intro; intros.
+- simpl in H14.
+  rewrite map_rev.
+  assumption.
+- constructor.
+- intro; intros.
   destruct (Hch2o S'); try tauto.
-  apply rtc_transitive with (2:=H1).
+  apply rtc_transitive with (2:=H4).
   (* Showing a CH2O execution *)
   (* Calling main *)
   eapply rtc_l. {
@@ -1050,70 +3096,91 @@ eapply stmt_soundness; try eassumption. {
     - reflexivity.
   }
   simpl.
+  rewrite rev_length.
   apply rtc_refl.
-} {
-  intros.
-  destruct (H2 (State [] (Return "main" voidV) ∅)). {
+- intros.
+  destruct (H4 (State [] (Return "main" voidV) m')). {
     eapply rtc_l; [|apply rtc_refl].
     constructor.
   }
-  - inversion H4.
-  - destruct H4 as [S'' H4].
-    inversion H4.
-}
-intros.
-intro; intros.
-inversion H7; clear H7; subst. {
-  right.
-  eexists; eexists.
-  right.
-  constructor.
-  - simpl.
-    apply sem_cast_int.
-  - reflexivity.
-}
-inversion H8; clear H8; subst; inversion H7; clear H7; subst. {
-  inversion H17; clear H17; subst; try discriminate.
-} {
-  inversion H17; clear H17; subst; try discriminate.
-  subst.
-  inversion H16.
-} {
-  inversion H17; clear H17; subst; try discriminate.
-  subst.
-  inversion H16.
-} {
-  inversion H16; clear H16; subst; try discriminate.
-  subst.
-  elim H17.
-  constructor.
-}
-rewrite H4 in H9.
-simpl in H9.
-inversion H9; clear H9; subst. 2:{
-  inversion H7; clear H7; subst; inversion H9; clear H9; subst.
-}
-left.
-simpl in H17.
-rewrite sem_cast_int in H17.
-injection H17; clear H17; intros; subst.
-constructor.
-rewrite Int.signed_repr. 2:{
-  apply int_typed_limits; assumption.
-}
-(* Proving Q z *)
-destruct (H5 (state.State [] (Return "main" (intV{sintT} z)) ∅)). 2:{
-  inversion H7; assumption.
-} 2:{
-  destruct H7.
-  inversion H7.
-}
-(* Finishing executing ret *)
-eapply rtc_l. {
-  constructor.
-}
-simpl.
-apply rtc_refl.
+  + inversion H6.
+  + destruct H6 as [S'' H6].
+    inversion H6.
+- intros.
+  intro; intros.
+  edestruct free_list_lemma as [ṁ'' ?]; try eassumption.
+  + intros.
+    apply elem_of_list_In.
+    apply <- In_rev.
+    rewrite rev_involutive.
+    apply elem_of_list_In.
+    eapply Henv_tight.
+    eassumption.
+  + apply Maps.PTree.elements_keys_norepet.
+  + intros.
+    clear b H1 H3.
+    destruct xbτ as [x [b τ]].
+    split.
+    * apply Maps.PTree.elements_complete; eassumption.
+    * pose proof (H10 x).
+      apply Maps.PTree.elements_complete in H16.
+      unfold Values.block in H1.
+      rewrite H16 in H1.
+      apply H1.
+      apply Henv_tight in H16.
+      apply elem_of_list_In in H16.
+      assumption.
+  + inversion H15; clear H15; subst. {
+      right.
+      eexists; eexists.
+      right.
+      constructor.
+      - simpl.
+        apply sem_cast_int.
+      - apply H16.
+    }
+    inversion H17; clear H17; subst; inversion H15; clear H15; subst. {
+      inversion H26; clear H26; subst; try discriminate.
+    } {
+      inversion H26; clear H26; subst; try discriminate.
+      subst.
+      inversion H25.
+    } {
+      inversion H26; clear H26; subst; try discriminate.
+      subst.
+      inversion H25.
+    } {
+      inversion H25; clear H25; subst; try discriminate.
+      subst.
+      elim H26.
+      constructor.
+    }
+    rewrite H8 in H18.
+    simpl in H18.
+    inversion H18; clear H18; subst. 2:{
+      inversion H15; clear H15; subst; inversion H18; clear H18; subst.
+    }
+    left.
+    simpl in H26.
+    rewrite sem_cast_int in H26.
+    injection H26; clear H26; intros; subst.
+    constructor.
+    rewrite Int.signed_repr. 2:{
+      apply int_typed_limits; assumption.
+    }
+    (* Proving Q z *)
+    destruct (H12 (state.State [] (Return "main" (intV{sintT} z)) m')). 2:{
+      inversion H15; assumption.
+    } 2:{
+      destruct H15.
+      inversion H15.
+    }
+    (* Finishing executing ret *)
+    eapply rtc_l. {
+      constructor.
+    }
+    simpl.
+    apply rtc_refl.
 Qed.
 
 End Program.
