ch2o_bigstep/bigstep_soundness.v
@@ -266,6 +266,190 @@ induction 1.
     rewrite assert_eval_int_cast with (τi:=sintT%IT) (σi:=sintT%IT).
     * rewrite int_cast_self; [|assumption]. reflexivity.
     * apply int_cast_ok_self; assumption.
+- eapply ax_stmt_weaken_post with (Q:=(assert_stack (<[i:=Some z]>st))%A). {
+    apply assert_exist_intro with (x:=(<[i:=Some z]> st)).
+    rewrite assert_Prop_r; reflexivity.
+  }
+  eapply ax_stmt_weaken_pre with (P:=((∃p, var i ⇓ inl p ∧ emp) ★ assert_stack st)%A). {
+    apply assert_stack_var.
+    assumption.
+  }
+  apply ax_do.
+  apply ax_cast with (Q1:=(λ v, ⌜ v = inr (intV{sintT} z) /\ int_typed z sintT%IT ⌝ ★ assert_stack (<[i:=Some z]> st) ◊)%A). {
+    intros.
+    apply assert_Prop_intro_l.
+    intros.
+    destruct H1.
+    injection H1; clear H1; intros; subst.
+    eapply assert_exist_intro.
+    eapply assert_and_intro. { reflexivity. }
+    eapply assert_wand_intro.
+    unfold subseteqE.
+    unfold assert_entails.
+    intros.
+    unfold assert_holds.
+    unfold assert_expr.
+    eexists.
+    split. {
+      econstructor.
+      - econstructor.
+        + apply lockset_empty_valid.
+        + constructor.
+          constructor.
+          constructor.
+          assumption.
+      - constructor.
+        constructor.
+      - constructor.
+        constructor.
+    }
+    simpl.
+    rewrite option_guard_True; [|reflexivity].
+    simpl.
+    reflexivity.
+  }
+  eapply ax_expr_weaken_pre. {
+    apply assert_sep_preserving. reflexivity.
+    eapply assert_Prop_True.
+    apply assert_stack_typed.
+  }
+  eapply ax_expr_weaken_pre. {
+    apply (commutative (★)%A).
+  }
+  eapply ax_expr_weaken_pre. {
+    rewrite <- (associative (★)%A).
+    reflexivity.
+  }
+  apply ax_expr_Prop_pre; intros Hstore_typed.
+  eapply ax_expr_weaken_pre. {
+    rewrite (commutative (★)%A).
+    reflexivity.
+  }
+  apply ax_assign with
+    (Q1:=λ ν, (var i ⇓ ν ∧ emp)%A)
+    (Q2:=λ ν, (⌜ν = inr (intV{sintT} z) ∧ int_typed z sintT⌝ ★ assert_stack st)%A)
+    (μ:=false)
+    (γ:=perm_full)
+    (τ:=sintT%T).
+  + reflexivity.
+  + intros.
+    rewrite (commutative (★)%A).
+    rewrite <- (associative (★)%A).
+    apply assert_Prop_intro_l. intros. destruct H1 as [H1 Hz].
+    injection H1; clear H1; intros; subst.
+    rewrite (commutative (★)%A).
+    apply assert_exist_intro with (x:=intV{sintT} z).
+    apply assert_exist_intro with (x:=intV{sintT} z).
+    apply assert_and_intro.
+    * clear H0 Hstore_typed.
+      revert st i H.
+      induction st.
+      -- simpl; intros; lia.
+      -- Opaque perm_full.
+         rename a into mv.
+         simpl; intros.
+         destruct i.
+         ++ clear IHst H.
+            simpl.
+            assert (var_points_to 0 mv ⊆{Γ,δ} var 0 ↦{false,perm_full} - : sintT%BT)%A. {
+              destruct mv.
+              - eapply assert_exist_intro.
+                simpl. reflexivity.
+              - reflexivity.
+            }
+            rewrite H.
+            rewrite assert_singleton_l_.
+            rewrite (commutative (★)%A).
+            rewrite <- (associative (★)%A).
+            rewrite assert_exist_sep.
+            apply assert_exist_elim; intro p'.
+            rewrite (associative (★)%A).
+            rewrite (commutative (★)%A).
+            rewrite <- (associative (★)%A).
+            rewrite (associative (★)%A).
+            rewrite assert_eval_functional'.
+            rewrite <- (associative (★)%A).
+            apply assert_Prop_intro_l. intro Hp'. injection Hp'; clear Hp'; intros; subst p'.
+            rewrite (associative (★)%A).
+            rewrite (commutative (★)%A).
+            rewrite (associative (★)%A).
+            rewrite (commutative (★)%A).
+            apply assert_sep_preserving; [reflexivity|].
+            rewrite (commutative (★)%A).
+            apply assert_wand_intro.
+            rewrite assert_Prop_l. 2:{ tauto. }
+            rewrite (commutative (★)%A).
+            rewrite (associative (★)%A).
+            rewrite <- assert_unlock_sep.
+            apply assert_sep_preserving.
+            ** rewrite (commutative (★)%A).
+               rewrite assert_singleton_l_2.
+               apply assert_unlock_singleton.
+               reflexivity.
+            ** apply assert_stack_unlock_indep.
+         ++ simpl.
+            rewrite <- assert_unlock_sep.
+            rewrite <- assert_wand_sep.
+            rewrite <- assert_wand_sep.
+            rewrite (commutative (★)%A).
+            rewrite <- (associative (★)%A).
+            rewrite (commutative (★)%A) with (x:=(% p ↦{false,perm_full} - : sintT%BT)%A).
+            rewrite <- (associative (★)%A).
+            rewrite assert_Prop_l. 2:{ tauto. }
+            rewrite <- (associative (★)%A).
+            apply assert_sep_preserving; [apply var_points_to_unlock_indep|].
+            rewrite (commutative (★)%A).
+            rewrite (commutative (★)%A) with (y:=(% p ↦{false,perm_full} - : sintT%BT)%A).
+            assert (
+              ((var (S i) ⇓ inl p ∧ emp) ★ assert_stack st↑)%A ⊆{Γ,δ}
+              (((var i ⇓ inl p ∧ emp) ★ assert_stack st)↑)%A). {
+              rewrite assert_lift_sep.
+              rewrite assert_lift_and.
+              rewrite stack_indep.
+              apply assert_sep_preserving; [|reflexivity].
+              apply assert_and_intro.
+              - apply assert_and_elim_l.
+                rewrite <- assert_lift_eval.
+                reflexivity.
+              - apply assert_and_elim_r; reflexivity.
+            }
+            rewrite H0.
+            rewrite IHst.
+            ** rewrite assert_lift_sep.
+               rewrite assert_lift_wand.
+               rewrite assert_Prop_l. 2:{ tauto. }
+               rewrite assert_lift_unlock.
+               rewrite assert_lift_singleton.
+               rewrite assert_lift_singleton_.
+               reflexivity.
+            ** lia.
+    * apply assert_wand_intro.
+      simpl.
+      rewrite eval_sound with (1:=H0).
+      assert (forall P Q, P ⊆{Γ,δ} Q -> P ⊆{Γ,δ} (Q ∧ Q)%A). {
+        intros.
+        apply assert_and_intro; assumption.
+      }
+      apply H1; clear H1.
+      rewrite (right_id _ (★)%A).
+      rewrite <- (left_id _ (★)%A) with (x:=(cast{sintT%BT} (# intV{sintT} z) ⇓ inr (intV{sintT} z))%A).
+      apply assert_sep_preserving.
+      -- apply assert_and_elim_r; reflexivity.
+      -- rewrite assert_eval_int_typed.
+         apply assert_Prop_intro_l. intro Hz'.
+         eapply assert_eval_int_cast'.
+         ++ rewrite <- assert_int_typed_eval; trivial.
+         ++ apply int_cast_ok_self; apply Hz'.
+         ++ apply int_cast_self; assumption.
+  + apply ax_expr_exist_pre. intro p.
+    apply ax_expr_base with (ν:=inl p).
+    apply assert_and_intro; [reflexivity|].
+    apply assert_and_elim_l; reflexivity.
+  + apply ax_expr_base with (ν:=inr (intV{sintT} z)).
+    rewrite assert_Prop_l. 2:{ split. reflexivity. eapply eval_typed; eassumption. }
+    apply assert_and_intro; [reflexivity|].
+    rewrite eval_sound with (1:=H0) at 1.
+    reflexivity.
 - eapply ax_comp with (P':=assert_stack st').
   + eapply ax_stmt_weaken.
     Focus 8. {
